Test/FarmerGooseFoxChecker.lean
@@ -1,19 +1,22 @@
 import Veil
 import Veil.Frontend.DSL.Action.Extraction.Extract
 import Veil.Core.Tools.Checker.Concrete.Main
+
+import Veil.Core.Tools.Checker.Concrete.modelCheckerView
+import ProofWidgets.Component.HtmlDisplay
 -- -------------------------- MODULE FarmerGooseFox  --------------------------
 -- Source: https://gitlab.com/hhan31/rivercrossing-tla/-/blob/main/FarmerGooseFox.tla?ref_type=heads
 
 veil module FarmerGooseFox
 
--- type a
 
-relation Here : Bool
-relation There : Bool
-relation farmer : Bool
-relation beans : Bool
-relation goose : Bool
-relation fox : Bool
+
+individual Here : Bool
+individual There : Bool
+individual farmer : Bool
+individual beans : Bool
+individual goose : Bool
+individual fox : Bool
 
 #gen_state
 
@@ -57,154 +60,221 @@ action Withfox {
 }
 
 invariant [Unsolved] ¬ (farmer = There ∧ beans = There ∧ goose = There ∧ fox = There)
+termination [test] ¬ (farmer = There ∧ beans = There ∧ goose = There ∧ fox = There)
+
 #gen_spec
 
--- a syntax for filling sort arguments
-open Lean Meta Elab Command Veil in
-scoped elab "⌞? " t:term " ⌟" : term => do
-  let lenv ← localEnv.get
-  let some mod := lenv.currentModule | throwError s!"Not in a module"
-  Term.elabTerm (← `(term| $t $(← mod.sortIdents)*)) none
 
--- #time #check_invariants
 section
 
 veil_variables
 
 omit χ χ_rep χ_rep_lawful
 
-open Veil
+open Veil Extract
 
-variable [FinEnum node] [Hashable node]
--- variable [insta : DecidableRel tot.le] -- [∀ a b c, Decidable (btwn.btw a b c)]
+deriving_FinOrdToJson_Domain
 
-def instFinEnumForComponents (f : State.Label)
-  : (IteratedProd <| List.map FinEnum <| (⌞? State.Label.toDomain ⌟) f) := by
-  cases f <;>
-    infer_instance_for_iterated_prod
+specify_FieldConcreteType
 
-instance instDecidableEqForComponents' (f : State.Label)
-  : DecidableEq (IteratedProd <| (⌞? State.Label.toDomain ⌟) f) := by
-  cases f <;>
-    dsimp only [IteratedProd, List.foldr, State.Label.toDomain] <;>
-    infer_instance
+deriving_BEq_FieldConcreteType
 
-instance instDecidableEqForComponents'' (f : State.Label)
-  : DecidableEq (IteratedProd' <| (⌞? State.Label.toDomain ⌟) f) := by
-  cases f <;>
-    dsimp only [IteratedProd', State.Label.toDomain] <;>
-    infer_instance
+deriving_Hashable_FieldConcreteType
 
-instance instHashableForComponents (f : State.Label)
-  : Hashable (IteratedProd <| (⌞? State.Label.toDomain ⌟) f) := by
-  cases f <;>
-    dsimp only [IteratedProd, List.foldr, State.Label.toDomain] <;>
-    infer_instance
+deriving_rep_FieldRepresentation
 
-instance instHashableForComponents' (f : State.Label)
-  : Hashable (IteratedProd' <| (⌞? State.Label.toDomain ⌟) f) := by
-  cases f <;>
-    dsimp only [IteratedProd', State.Label.toDomain] <;>
-    infer_instance
+deriving_lawful_FieldRepresentation
 
+deriving_Inhabited_State
 
--- need to use `abbrev` to allow typeclass inference
-abbrev FieldConcreteType (f : State.Label) : Type :=
-  match f with
-  | State.Label.Here => Std.HashSet (IteratedProd' <| (⌞? State.Label.toDomain ⌟) State.Label.Here)
-  | State.Label.There => Std.HashSet (IteratedProd' <| (⌞? State.Label.toDomain ⌟) State.Label.There)
-  | State.Label.farmer => Std.HashSet (IteratedProd' <| (⌞? State.Label.toDomain ⌟) State.Label.farmer)
-  | State.Label.beans => Std.HashSet (IteratedProd' <| (⌞? State.Label.toDomain ⌟) State.Label.beans)
-  | State.Label.goose => Std.HashSet (IteratedProd' <| (⌞? State.Label.toDomain ⌟) State.Label.goose)
-  | State.Label.fox => Std.HashSet (IteratedProd' <| (⌞? State.Label.toDomain ⌟) State.Label.fox)
-
-instance instReprForComponents (f : State.Label)
-  : Repr ((⌞? FieldConcreteType ⌟) f) := by
-  cases f <;>
-    dsimp only [IteratedProd, IteratedProd', List.foldr, FieldConcreteType, State.Label.toDomain] <;>
-    infer_instance
-
--- #simp [FieldConcreteType, State.Label.toDomain, State.Label.toCodomain] FieldConcreteType Nat .leader
-  -- Veil.CanonicalField (State.Label.toDomain Nat .pending) (State.Label.toCodomain Nat .pending)
-
-instance : Inhabited ((⌞? State ⌟) (⌞? FieldConcreteType ⌟)) := by
-  constructor ; constructor <;> exact default
-
-instance rep (f : State.Label) : FieldRepresentation
-  ((⌞? State.Label.toDomain ⌟) f)
-  ((⌞? State.Label.toCodomain ⌟) f)
-  ((⌞? FieldConcreteType ⌟) f) :=-- by cases f <;> apply instFinsetLikeAsFieldRep <;> apply instFinEnumForComponents
-  match f with
-  | State.Label.Here =>
-    instFinsetLikeAsFieldRep (IteratedProd'.equiv) ((⌞? instFinEnumForComponents ⌟) State.Label.Here)
-  | State.Label.There =>
-    instFinsetLikeAsFieldRep (IteratedProd'.equiv) ((⌞? instFinEnumForComponents ⌟) State.Label.There)
-  | State.Label.farmer =>
-    instFinsetLikeAsFieldRep (IteratedProd'.equiv) ((⌞? instFinEnumForComponents ⌟) State.Label.farmer)
-  | State.Label.beans =>
-    instFinsetLikeAsFieldRep (IteratedProd'.equiv) (( ⌞? instFinEnumForComponents ⌟) State.Label.beans)
-  | State.Label.goose =>
-    instFinsetLikeAsFieldRep (IteratedProd'.equiv) ((⌞? instFinEnumForComponents ⌟) State.Label.goose)
-  | State.Label.fox =>
-    instFinsetLikeAsFieldRep (IteratedProd'.equiv) ((⌞? instFinEnumForComponents ⌟) State.Label.fox)
-
-instance lawful (f : State.Label) : LawfulFieldRepresentation
-  ((⌞? State.Label.toDomain ⌟) f)
-  ((⌞? State.Label.toCodomain ⌟) f)
-  ((⌞? FieldConcreteType ⌟) f)
-  ((⌞? rep ⌟) f) :=-- by cases f <;> apply instFinsetLikeAsFieldRep <;> apply instFinEnumForComponents
-  match f with
-  | State.Label.Here =>
-    instFinsetLikeLawfulFieldRep (IteratedProd'.equiv) ((⌞? instFinEnumForComponents ⌟) State.Label.Here)
-  | State.Label.There =>
-    instFinsetLikeLawfulFieldRep (IteratedProd'.equiv) ((⌞? instFinEnumForComponents ⌟) State.Label.There)
-  | State.Label.farmer =>
-    instFinsetLikeLawfulFieldRep (IteratedProd'.equiv) ((⌞? instFinEnumForComponents ⌟) State.Label.farmer)
-  | State.Label.beans =>
-    instFinsetLikeLawfulFieldRep (IteratedProd'.equiv   ) ((⌞? instFinEnumForComponents ⌟) State.Label.beans)
-  | State.Label.goose =>
-    instFinsetLikeLawfulFieldRep (IteratedProd'.equiv) ((⌞? instFinEnumForComponents ⌟) State.Label.goose)
-  | State.Label.fox =>
-    instFinsetLikeLawfulFieldRep (IteratedProd'.equiv) ((⌞? instFinEnumForComponents ⌟) State.Label.fox)
+deriving_Decidable_Props
 
 end
 
--- code optimization by controlled `dsimp`
--- set_option trace.Compiler.result true in
-attribute [local dsimpFieldRepresentationGet, local dsimpFieldRepresentationSet]
-  instFinEnumForComponents in
--- attribute [local dsimpFieldRepresentationGet] FourNodes.equiv_IteratedProd in
-#specialize_nextact with FieldConcreteType
-  injection_begin injection_end => NextAct'
+gen_NextAct
 
-#gen_executable_list! log_entry_being Std.Format
-  targeting NextAct'
-  injection_begin  injection_end
+gen_executable_NextAct
 
-
-simple_deriving_repr_for' State
-deriving instance Repr for Label
-deriving instance Inhabited for Theory
-
-instance [Hashable α] [BEq α] : Hashable (Std.HashSet α) where
-  hash s :=
-    /- `Hash collision `-/
-    s.fold (init := 0) fun acc a => acc + (hash a)
 
 #Concretize
-#assembleInsts
 
-instance : (rd : TheoryConcrete) → (st : StateConcrete) → Decidable ((fun ρ σ => Unsolved ρ σ) rd st) :=
-  by
-  intro rd st
-  dsimp [Unsolved]
-  dsimp [FieldConcreteType, State.Label.toDomain, State.Label.toCodomain]
-  infer_instance
+deriving_BEqHashable_ConcreteState
+-- deriving instance Inhabited for Theory
+
+-- a syntax for filling sort arguments
+-- open Lean Meta Elab Command Veil in
+-- scoped elab "⌞? " t:term " ⌟" : term => do
+--   let lenv ← localEnv.get
+--   let some mod := lenv.currentModule | throwError s!"Not in a module"
+--   Term.elabTerm (← `(term| $t $(← mod.sortIdents)*)) none
 
 
-def modelCheckerResult' := (runModelCheckerx initVeilMultiExecM nextVeilMultiExecM labelList (fun ρ σ => Unsolved ρ σ) {} id).snd
-#time #eval modelCheckerResult'
-#html createExpandedGraphDisplay (collectTrace modelCheckerResult').1 (collectTrace modelCheckerResult').2
+-- @[derivedInvSimp, invSimp, reducible]
+-- def Invariants (ρ : Type) (σ : Type) (χ : State.Label → Type)
+--     [χ_rep : ∀ f, Veil.FieldRepresentation (State.Label.toDomain f) (State.Label.toCodomain f) (χ f)]
+--     [χ_rep_lawful :
+--       ∀ f, Veil.LawfulFieldRepresentation (State.Label.toDomain f) (State.Label.toCodomain f) (χ f) (χ_rep f)]
+--     [σ_sub : IsSubStateOf @State χ σ] [ρ_sub : IsSubReaderOf @Theory ρ] (rd : ρ) (st : σ) : Prop :=
+--   @Unsolved ρ σ χ χ_rep χ_rep_lawful σ_sub ρ_sub rd st
+
+-- #time #check_invariants
+-- #exit
+-- section
+-- veil_variables
+
+-- omit χ χ_rep χ_rep_lawful
+
+-- open Veil
+
+-- variable [FinEnum node] [Hashable node]
+-- -- variable [insta : DecidableRel tot.le] -- [∀ a b c, Decidable (btwn.btw a b c)]
+
+-- def instFinEnumForComponents (f : State.Label)
+--   : (IteratedProd <| List.map FinEnum <| (⌞? State.Label.toDomain ⌟) f) := by
+--   cases f <;>
+--     infer_instance_for_iterated_prod
+
+-- instance instDecidableEqForComponents' (f : State.Label)
+--   : DecidableEq (IteratedProd <| (⌞? State.Label.toDomain ⌟) f) := by
+--   cases f <;>
+--     dsimp only [IteratedProd, List.foldr, State.Label.toDomain] <;>
+--     infer_instance
+
+-- instance instDecidableEqForComponents'' (f : State.Label)
+--   : DecidableEq (IteratedProd' <| (⌞? State.Label.toDomain ⌟) f) := by
+--   cases f <;>
+--     dsimp only [IteratedProd', State.Label.toDomain] <;>
+--     infer_instance
+
+-- instance instHashableForComponents (f : State.Label)
+--   : Hashable (IteratedProd <| (⌞? State.Label.toDomain ⌟) f) := by
+--   cases f <;>
+--     dsimp only [IteratedProd, List.foldr, State.Label.toDomain] <;>
+--     infer_instance
+
+-- instance instHashableForComponents' (f : State.Label)
+--   : Hashable (IteratedProd' <| (⌞? State.Label.toDomain ⌟) f) := by
+--   cases f <;>
+--     dsimp only [IteratedProd', State.Label.toDomain] <;>
+--     infer_instance
+
+
+-- -- need to use `abbrev` to allow typeclass inference
+-- abbrev FieldConcreteType (f : State.Label) : Type :=
+--   match f with
+--   | State.Label.Here => Std.HashSet (IteratedProd' <| (⌞? State.Label.toDomain ⌟) State.Label.Here)
+--   | State.Label.There => Std.HashSet (IteratedProd' <| (⌞? State.Label.toDomain ⌟) State.Label.There)
+--   | State.Label.farmer => Std.HashSet (IteratedProd' <| (⌞? State.Label.toDomain ⌟) State.Label.farmer)
+--   | State.Label.beans => Std.HashSet (IteratedProd' <| (⌞? State.Label.toDomain ⌟) State.Label.beans)
+--   | State.Label.goose => Std.HashSet (IteratedProd' <| (⌞? State.Label.toDomain ⌟) State.Label.goose)
+--   | State.Label.fox => Std.HashSet (IteratedProd' <| (⌞? State.Label.toDomain ⌟) State.Label.fox)
+
+-- instance instReprForComponents (f : State.Label)
+--   : Repr ((⌞? FieldConcreteType ⌟) f) := by
+--   cases f <;>
+--     dsimp only [IteratedProd, IteratedProd', List.foldr, FieldConcreteType, State.Label.toDomain] <;>
+--     infer_instance
+
+-- -- #simp [FieldConcreteType, State.Label.toDomain, State.Label.toCodomain] FieldConcreteType Nat .leader
+--   -- Veil.CanonicalField (State.Label.toDomain Nat .pending) (State.Label.toCodomain Nat .pending)
+
+-- instance : Inhabited ((⌞? State ⌟) (⌞? FieldConcreteType ⌟)) := by
+--   constructor ; constructor <;> exact default
+
+-- instance rep (f : State.Label) : FieldRepresentation
+--   ((⌞? State.Label.toDomain ⌟) f)
+--   ((⌞? State.Label.toCodomain ⌟) f)
+--   ((⌞? FieldConcreteType ⌟) f) :=-- by cases f <;> apply instFinsetLikeAsFieldRep <;> apply instFinEnumForComponents
+--   match f with
+--   | State.Label.Here =>
+--     instFinsetLikeAsFieldRep (IteratedProd'.equiv) ((⌞? instFinEnumForComponents ⌟) State.Label.Here)
+--   | State.Label.There =>
+--     instFinsetLikeAsFieldRep (IteratedProd'.equiv) ((⌞? instFinEnumForComponents ⌟) State.Label.There)
+--   | State.Label.farmer =>
+--     instFinsetLikeAsFieldRep (IteratedProd'.equiv) ((⌞? instFinEnumForComponents ⌟) State.Label.farmer)
+--   | State.Label.beans =>
+--     instFinsetLikeAsFieldRep (IteratedProd'.equiv) (( ⌞? instFinEnumForComponents ⌟) State.Label.beans)
+--   | State.Label.goose =>
+--     instFinsetLikeAsFieldRep (IteratedProd'.equiv) ((⌞? instFinEnumForComponents ⌟) State.Label.goose)
+--   | State.Label.fox =>
+--     instFinsetLikeAsFieldRep (IteratedProd'.equiv) ((⌞? instFinEnumForComponents ⌟) State.Label.fox)
+
+-- instance lawful (f : State.Label) : LawfulFieldRepresentation
+--   ((⌞? State.Label.toDomain ⌟) f)
+--   ((⌞? State.Label.toCodomain ⌟) f)
+--   ((⌞? FieldConcreteType ⌟) f)
+--   ((⌞? rep ⌟) f) :=-- by cases f <;> apply instFinsetLikeAsFieldRep <;> apply instFinEnumForComponents
+--   match f with
+--   | State.Label.Here =>
+--     instFinsetLikeLawfulFieldRep (IteratedProd'.equiv) ((⌞? instFinEnumForComponents ⌟) State.Label.Here)
+--   | State.Label.There =>
+--     instFinsetLikeLawfulFieldRep (IteratedProd'.equiv) ((⌞? instFinEnumForComponents ⌟) State.Label.There)
+--   | State.Label.farmer =>
+--     instFinsetLikeLawfulFieldRep (IteratedProd'.equiv) ((⌞? instFinEnumForComponents ⌟) State.Label.farmer)
+--   | State.Label.beans =>
+--     instFinsetLikeLawfulFieldRep (IteratedProd'.equiv   ) ((⌞? instFinEnumForComponents ⌟) State.Label.beans)
+--   | State.Label.goose =>
+--     instFinsetLikeLawfulFieldRep (IteratedProd'.equiv) ((⌞? instFinEnumForComponents ⌟) State.Label.goose)
+--   | State.Label.fox =>
+--     instFinsetLikeLawfulFieldRep (IteratedProd'.equiv) ((⌞? instFinEnumForComponents ⌟) State.Label.fox)
+
+-- end
+
+-- -- code optimization by controlled `dsimp`
+-- -- set_option trace.Compiler.result true in
+-- attribute [local dsimpFieldRepresentationGet, local dsimpFieldRepresentationSet]
+--   instFinEnumForComponents in
+-- -- attribute [local dsimpFieldRepresentationGet] FourNodes.equiv_IteratedProd in
+-- #specialize_nextact with FieldConcreteType
+--   injection_begin injection_end => NextAct'
+
+-- #gen_executable_list! log_entry_being Std.Format
+--   targeting NextAct'
+--   injection_begin  injection_end
+
+
+-- simple_deriving_repr_for' State
+-- deriving instance Repr for Label
+-- deriving instance Inhabited for Theory
+
+-- instance [Hashable α] [BEq α] : Hashable (Std.HashSet α) where
+--   hash s :=
+--     /- `Hash collision `-/
+--     s.fold (init := 0) fun acc a => acc + (hash a)
+
+-- #Concretize
+-- #assembleInsts
+
+-- instance : (rd : TheoryConcrete) → (st : StateConcrete) → Decidable ((fun ρ σ => Unsolved ρ σ) rd st) :=
+--   by
+--   intro rd st
+--   dsimp [Unsolved]
+--   dsimp [FieldConcreteType, State.Label.toDomain, State.Label.toCodomain]
+--   infer_instance
+
+
+
+-- def modelCheckerResult' := (runModelCheckerx initVeilMultiExecM nextVeilMultiExecM labelList (fun ρ σ => Unsolved ρ σ) ((fun ρ σ => true)) {} id).snd
+-- #time #eval modelCheckerResult'
+-- #html createExpandedGraphDisplay (collectTrace modelCheckerResult').1 (collectTrace modelCheckerResult').2
+
+-- simple_deriving_repr_for' State
+deriving instance Repr for Label
+-- deriving instance Inhabited for Theory
+
+deriving_toJson_for_state
+
+
+def modelCheckerResult' := (runModelCheckerx initVeilMultiExecM nextVeilMultiExecM labelList (fun ρ σ => Unsolved ρ σ) ((fun ρ σ => true)) {} hash).snd
+
+
+def statesJson : Lean.Json :=
+  Lean.toJson (recoverTrace initVeilMultiExecM nextVeilMultiExecM {} (collectTrace' modelCheckerResult'))
+open ProofWidgets
+open scoped ProofWidgets.Jsx
+#html <ModelCheckerView trace={statesJson} layout={"vertical"} />
+
+
 
 
 end FarmerGooseFox
