Examples/modelChecker/Bakery.lean
@@ -1,0 +1,139 @@
+import Veil
+import Veil.Frontend.DSL.Action.Extraction.Extract
+import Veil.Core.Tools.Checker.Concrete.Main
+
+import Veil.Core.Tools.Checker.Concrete.modelCheckerView
+import ProofWidgets.Component.HtmlDisplay
+
+veil module SimpleAllocator
+-- ------------------------ MODULE SimpleAllocator -------------------------
+-- (***********************************************************************)
+-- (* Specification of an allocator managing a set of resources:          *)
+-- (* - Clients can request sets of resources whenever all their previous *)
+-- (*   requests have been satisfied.                                     *)
+-- (* - Requests can be partly fulfilled, and resources can be returned   *)
+-- (*   even before the full request has been satisfied. However, clients *)
+-- (*   only have an obligation to return resources after they have       *)
+-- (*   obtained all resources they requested.                            *)
+-- (***********************************************************************)
+-- https://github.com/tlaplus/Examples/blob/master/specifications/allocator/SimpleAllocator.tla
+
+-- EXTENDS FiniteSets, TLC
+
+-- CONSTANTS
+--   Clients,     \* set of all clients
+--   Resources    \* set of all resources
+type client
+type resource
+immutable relation Clients : client → Bool
+immutable relation Resources : resource → Bool
+-- ASSUME
+--   IsFiniteSet(Resources)
+
+-- VARIABLES
+--   unsat,       \* set of all outstanding requests per process
+--   alloc        \* set of resources allocated to given process
+relation unsatisfy : client → resource → Bool
+relation alloc : client → resource → Bool
+-- TypeInvariant ==
+--   /\ unsat \in [Clients -> SUBSET Resources]
+--   /\ alloc \in [Clients -> SUBSET Resources]
+
+-- -------------------------------------------------------------------------
+#gen_state
+assumption [fixed_clients_set] ∀c, Clients c
+assumption [finite_resources] ∀s, Resources s
+
+
+after_init {
+  unsatisfy C R := false
+  alloc C R := false
+}
+
+
+action Request (c : client) (s : resource) {
+  require ∀r, ¬ unsatisfy c r
+  require ∀r, ¬ alloc c r
+  -- require ¬ S # {}
+  unsatisfy c s := true
+}
+
+
+action Allocate (c : client) (s : resource) {
+  require unsatisfy c s ∧ (Resources s ∧ ∀c', ¬ alloc c' s)
+  -- Introduce an error here, originally is unsatisfy c s ∧ (Resources s ∧ ∀c', ¬ alloc c' s)
+  alloc c s := true
+  unsatisfy c s := false
+}
+
+
+action Return (c : client) (s : resource) {
+  require alloc c s
+  alloc c s := false
+}
+
+-- -------------------------------------------------------------------------
+
+-- (* The complete high-level specification. *)
+-- SimpleAllocator ==
+--   /\ Init /\ [][Next]_vars
+--   /\ \A c \in Clients: WF_vars(Return(c, alloc[c]))
+--   /\ \A c \in Clients: SF_vars(\E S \in SUBSET Resources: Allocate(c,S))
+
+-- -------------------------------------------------------------------------
+
+-- ResourceMutex ==
+--   \A c1,c2 \in Clients : c1 # c2 => alloc[c1] \cap alloc[c2] = {}
+invariant [resource_mutex] ∀c1 c2, c1 ≠ c2 → ¬(∃s, alloc c1 s ∧ alloc c2 s)
+-- ClientsWillReturn ==
+--   \A c \in Clients : unsat[c]={} ~> alloc[c]={}
+-- ClientsWillObtain ==
+--   \A c \in Clients, r \in Resources : r \in unsat[c] ~> r \in alloc[c]
+-- InfOftenSatisfied ==
+--   \A c \in Clients : []<>(unsat[c] = {})
+
+-- -------------------------------------------------------------------------
+
+-- (* Used for symmetry reduction with TLC *)
+-- Symmetry == Permutations(Clients) \cup Permutations(Resources)
+
+-- -------------------------------------------------------------------------
+
+-- (* The following version states a weaker fairness requirement for the  *)
+-- (* clients: resources need be returned only if the entire request has  *)
+-- (* been satisfied.                                                     *)
+
+-- SimpleAllocator2 ==
+--   /\ Init /\ [][Next]_vars
+--   /\ \A c \in Clients: WF_vars(unsat[c] = {} /\ Return(c, alloc[c]))
+--   /\ \A c \in Clients: SF_vars(\E S \in SUBSET Resources: Allocate(c,S))
+
+#gen_spec
+-- #check_invariants
+
+-- -------------------------------------------------------------------------
+
+-- THEOREM SimpleAllocator => []TypeInvariant
+-- THEOREM SimpleAllocator => []ResourceMutex
+-- THEOREM SimpleAllocator => ClientsWillReturn
+-- THEOREM SimpleAllocator2 => ClientsWillReturn
+-- THEOREM SimpleAllocator => ClientsWillObtain
+-- THEOREM SimpleAllocator => InfOftenSatisfied
+-- (** The following do not hold:                          **)
+-- (** THEOREM SimpleAllocator2 => ClientsWillObtain       **)
+-- (** THEOREM SimpleAllocator2 => InfOftenSatisfied       **)
+-- =========================================================================
+#prepareExecution
+
+#finitizeTypes (Fin 5), (Fin 3)
+
+
+def modelCheckerResult' := (runModelCheckerx initVeilMultiExecM nextVeilMultiExecM labelList (fun ρ σ => resource_mutex ρ σ) ((fun ρ σ => true)) default hash).snd
+def statesJson : Lean.Json := Lean.toJson (recoverTrace initVeilMultiExecM nextVeilMultiExecM default (collectTrace' modelCheckerResult'))
+#eval modelCheckerResult'.seen.size
+open ProofWidgets
+open scoped ProofWidgets.Jsx
+#html <ModelCheckerView trace={statesJson} layout={"vertical"} />
+
+
+end SimpleAllocator
