Examples/modelChecker/Diehard.lean
@@ -1,0 +1,82 @@
+import Veil
+import Veil.Frontend.DSL.Action.Extraction.Extract
+import Veil.Core.Tools.Checker.Concrete.Main
+import ProofWidgets.Component.HtmlDisplay
+
+veil module DieHard
+
+individual big : Nat
+individual small : Nat
+
+#gen_state
+
+after_init {
+  big := 0
+  small := 0
+}
+
+
+action FillSmallJug {
+  small := 3
+  big := big
+}
+
+
+action FillBigJug  {
+  big := 5
+  small := small
+}
+
+
+action EmptySmallJug {
+  small := 0
+  big := big
+}
+
+
+action EmptyBigJug {
+  big := 0
+  small := small
+}
+
+
+action SmallToBig {
+  let tmp := big
+  big := if big + small < 5 then big + small else 5
+  small := small - (big - tmp)
+}
+
+
+
+action BigToSmall {
+  let tmp := small
+  small := if big + small < 3 then big + small else 3
+  big := big - (small - tmp)
+}
+
+
+invariant [typeOK] small≤ 3 ∧ big ≤ 5
+
+
+invariant [not_solved] big ≠ 4
+
+#gen_spec
+
+
+#time #check_invariants
+
+
+#prepareExecution
+
+#finitizeTypes
+
+
+def modelCheckerResult' := (runModelCheckerx initVeilMultiExecM nextVeilMultiExecM labelList (fun ρ σ => not_solved ρ σ) ((fun ρ σ => true)) {} hash).snd
+def statesJson : Lean.Json :=Lean.toJson (recoverTrace initVeilMultiExecM nextVeilMultiExecM {} (collectTrace' modelCheckerResult'))
+open ProofWidgets
+open scoped ProofWidgets.Jsx
+#html <ModelCheckerView trace={statesJson} layout={"vertical"} />
+
+
+
+end DieHard
