Examples/modelChecker/keyValueStore.lean
@@ -1,0 +1,200 @@
+import Veil
+import Veil.Frontend.DSL.Action.Extraction.Extract
+import Veil.Core.Tools.Checker.Concrete.Main
+
+import Veil.Core.Tools.Checker.Concrete.modelCheckerView
+import ProofWidgets.Component.HtmlDisplay
+/-
+Key-Value Store with Snapshot Isolation
+
+This module specifies a simple key-value store that exhibits snapshot isolation.
+In snapshot isolation, each transaction sees a consistent snapshot of the database
+as it existed at the start of the transaction.
+
+TLA⁺ Specification Author: Andrew Helwer
+
+Key Properties:
+- If two concurrent transactions write to the same key, the one committing later
+  will be rejected (write-write conflict detection)
+- If they write to different keys, both transactions will succeed
+- Each transaction operates on its own snapshot of the store
+- Write conflicts are detected by tracking which keys each transaction has written
+  and which writes it has "missed" from other concurrent transactions
+
+For a more detailed TLA⁺ specification of snapshot isolation, see:
+https://github.com/tlaplus/Examples/blob/master/specifications/KeyValueStore/KeyValueStore.tla
+-/
+veil module KeyValueStore
+
+/- Constants -/
+-- type key    -- The set of all keys.
+enum key = {K1, K2}
+-- type value  -- The set of all values.
+enum value = {noVal, v1, v2}
+-- type txId   -- The set of all transaction IDs.
+enum txId = {T1, T2}
+
+
+
+/- Variables -/
+-- A data store mapping keys to values.
+relation store : key → value → Bool
+-- The set of open snapshot transactions.
+relation tx : txId → Bool
+-- Snapshots of the store for each transaction.
+relation snapshotStore : txId → key → value → Bool
+-- A log of writes performed within each transaction.
+relation written : txId → key → Bool
+-- The set of writes invisible to each transaction.
+relation missed : txId → key → Bool
+-- Choose something to represent the absence of a value.
+-- immutable individual noVal : value
+
+#gen_state
+
+-- Init == \* The initial predicate.
+--     /\ store = [k \in Key |-> NoVal]        \* All store values are initially NoVal.
+--     /\ tx = {}                              \* The set of open transactions is initially empty.
+--     /\ snapshotStore =                      \* All snapshotStore values are initially NoVal.
+--         [t \in TxId |-> [k \in Key |-> NoVal]]
+--     /\ written = [t \in TxId |-> {}]        \* All write logs are initially empty.
+--     /\ missed = [t \in TxId |-> {}]         \* All missed writes are initially empty.
+after_init {
+  store K V := V == noVal
+  tx T := false
+  snapshotStore T K V := V == noVal
+  written T K := false
+  missed T K := false
+
+}
+
+
+-- OpenTx(t) ==    \* Open a new transaction.
+--     /\ t \notin tx
+--     /\ tx' = tx \cup {t}
+--     /\ snapshotStore' = [snapshotStore EXCEPT ![t] = store]
+--     /\ UNCHANGED <<written, missed, store>>
+action OpenTx (t : txId) {
+  require ¬ tx t
+  -- tx T := tx T ∨ t = T
+  tx t := true
+  snapshotStore t K V := store K V
+}
+
+-- Add(t, k, v) == \* Using transaction t, add value v to the store under key k.
+--     /\ t \in tx
+--     /\ snapshotStore[t][k] = NoVal
+--     /\ snapshotStore' = [snapshotStore EXCEPT ![t][k] = v]
+--     /\ written' = [written EXCEPT ![t] = @ \cup {k}]
+--     /\ UNCHANGED <<tx, missed, store>>
+action Add (t : txId) (k : key) (v : value)  {
+  require v ≠ noVal
+  require tx t
+  require snapshotStore t k noVal
+  snapshotStore t k V := V == v
+  written t k := true
+}
+
+-- Update(t, k, v) ==  \* Using transaction t, update the value associated with key k to v.
+--     /\ t \in tx
+--     /\ snapshotStore[t][k] \notin {NoVal, v}
+--     /\ snapshotStore' = [snapshotStore EXCEPT ![t][k] = v]
+--     /\ written' = [written EXCEPT ![t] = @ \cup {k}]
+--     /\ UNCHANGED <<tx, missed, store>>
+action Update (t : txId) (k : key) (v : value)  {
+  require v ≠ noVal
+  require tx t
+  require ¬ (snapshotStore t k noVal ∨ snapshotStore t k v)
+  snapshotStore t k V := decide $ V = v
+  written t k := true
+}
+
+-- Remove(t, k) == \* Using transaction t, remove key k from the store.
+--     /\ t \in tx
+--     /\ snapshotStore[t][k] /= NoVal
+--     /\ snapshotStore' = [snapshotStore EXCEPT ![t][k] = NoVal]
+--     /\ written' = [written EXCEPT ![t] = @ \cup {k}]
+--     /\ UNCHANGED <<tx, missed, store>>
+action Remove (t : txId) (k : key) {
+  require tx t
+  require ¬ snapshotStore t k noVal
+  snapshotStore t k V := decide $ V = noVal
+  written t k := true
+}
+
+
+-- RollbackTx(t) ==    \* Close the transaction without merging writes into store.
+--     /\ t \in tx
+--     /\ tx' = tx \ {t}
+--     /\ snapshotStore' = [snapshotStore EXCEPT ![t] = [k \in Key |-> NoVal]]
+--     /\ written' = [written EXCEPT ![t] = {}]
+--     /\ missed' = [missed EXCEPT ![t] = {}]
+--     /\ UNCHANGED store
+action RollbackTx (t : txId) {
+  require tx t
+  tx t := false
+  snapshotStore t K V :=  V == noVal
+  written t K := false
+  missed t K := false
+}
+
+
+
+
+-- CloseTx(t) ==   \* Close transaction t, merging writes into store.
+--     /\ t \in tx
+--     /\ missed[t] \cap written[t] = {}   \* Detection of write-write conflicts.
+--     /\ store' =                         \* Merge snapshotStore writes into store.
+--         [k \in Key |-> IF k \in written[t] THEN snapshotStore[t][k] ELSE store[k]]
+--     /\ tx' = tx \ {t}
+--     /\ missed' =    \* Update the missed writes for other open transactions.
+--         [otherTx \in TxId |-> IF otherTx \in tx' THEN missed[otherTx] \cup written[t] ELSE {}]
+--     /\ snapshotStore' = [snapshotStore EXCEPT ![t] = [k \in Key |-> NoVal]]
+--     /\ written' = [written EXCEPT ![t] = {}]
+action CloseTx (t : txId) (otherTx : txId) {
+  require tx t
+  require ¬(∃k, missed t k ∧ written t k)
+  store K V := if written t K then decide $ snapshotStore t K V else store K V
+  tx t := false
+  missed T K := if tx T then decide $ missed T K ∨ written t K else false
+  -- Here introduces error in the spec, originally is uncommented.
+  -- snapshotStore t K V := V == noVal
+  -- written t K := false
+}
+
+
+ghost relation snapshot_isolation :=
+  -- ∀t, tx t → (∀k, (∃v, store k v ≠ snapshotStore t k v ∧ ¬ written t k) → missed t k)
+  ∀t, tx t → (∀k, (∃v, store k v ≠ snapshotStore t k v ∧ ¬ written t k) → missed t k)
+
+ghost relation transaction_cleanup :=
+  ∀t, (¬tx t) → (∀k v, snapshotStore t k v → v = noVal) ∧
+  (∀k, ¬written t k) ∧ (∀k, ¬missed t k)
+invariant [unique_store] store K M ∧ store K N → M = N
+invariant [unique_snapshotStore] snapshotStore T K M ∧ snapshotStore T K N → M = N
+-- invariant [Txlifecycle] snapshot_isolation ∧ transaction_cleanup
+invariant [Txlifecycle] (  ∀t, tx t → (∀k, (∃v, store k v ≠ snapshotStore t k v ∧ ¬ written t k) → missed t k)) ∧
+  (∀t, (¬tx t) → (∀k v, snapshotStore t k v → v = noVal) ∧
+  (∀k, ¬written t k) ∧ (∀k, ¬missed t k))
+
+#gen_spec
+-- #time #check_invariants
+
+
+#prepareExecution
+
+#finitizeTypes key, value, txId
+-- #finitizeTypes (Fin 2), value, (Fin 2)
+
+
+
+def view (st : StateConcrete) := hash st
+def modelCheckerResult' :=(runModelCheckerx initVeilMultiExecM nextVeilMultiExecM labelList (fun ρ σ => Txlifecycle ρ σ) ((fun ρ σ => true)) {} view).snd
+#eval modelCheckerResult'.seen.size
+def statesJson : Lean.Json := Lean.toJson (recoverTrace initVeilMultiExecM nextVeilMultiExecM {} (collectTrace' modelCheckerResult'))
+open ProofWidgets
+open scoped ProofWidgets.Jsx
+#html <ModelCheckerView trace={statesJson} layout={"vertical"} />
+
+
+end KeyValueStore
