Examples/modelChecker/puzzle.lean
@@ -1,0 +1,103 @@
+import Veil
+import Veil.Frontend.DSL.Action.Extraction.Extract
+import Veil.Core.Tools.Checker.Concrete.Main
+import ProofWidgets.Component.HtmlDisplay
+
+veil module RiverCrossing
+
+enum position = {near, far}
+individual wolf_pos : position
+individual goat_pos : position
+individual cabbage_pos : position
+individual farmer_pos : position
+
+#print position_Enum
+-- enum act = {Init, FarmerAndWolf, FarmerAndGoat, FarmerAndCabbage, FarmerAlone}
+-- individual lastAction : act
+
+#gen_state
+
+/-
+Puzzle Rules:
+ * If goat and wolf are on the same bank p, the farmer must also be on p.
+ * If goat and cabbage are on the same bank p, the farmer must also be on p.
+-/
+ghost relation safety_constraint :=
+     (goat_pos = wolf_pos → farmer_pos = goat_pos) ∧
+     (goat_pos = cabbage_pos → farmer_pos = goat_pos)
+
+after_init {
+  wolf_pos := near
+  goat_pos := near
+  cabbage_pos := near
+  farmer_pos := near
+  -- lastAction := Init
+}
+
+action FarmerAndWolf {
+  require (goat_pos = wolf_pos → farmer_pos = goat_pos) ∧ (goat_pos = cabbage_pos → farmer_pos = goat_pos)
+  require farmer_pos = wolf_pos
+
+  if farmer_pos = far then
+    farmer_pos := near
+    wolf_pos := near
+  else
+    farmer_pos := far
+    wolf_pos := far
+  -- lastAction := FarmerAndWolf
+}
+
+action FarmerAndGoat {
+  require (goat_pos = wolf_pos → farmer_pos = goat_pos) ∧ (goat_pos = cabbage_pos → farmer_pos = goat_pos)
+  require farmer_pos = goat_pos
+  if farmer_pos = far then
+    farmer_pos := near
+    goat_pos := near
+  else
+    farmer_pos := far
+    goat_pos := far
+  -- lastAction := FarmerAndGoat
+}
+
+
+action FarmerAndCabbage {
+  require (goat_pos = wolf_pos → farmer_pos = goat_pos) ∧ (goat_pos = cabbage_pos → farmer_pos = goat_pos)
+  require farmer_pos = cabbage_pos
+  if farmer_pos = far then
+    farmer_pos := near
+    cabbage_pos := near
+  else
+    farmer_pos := far
+    cabbage_pos := far
+  -- lastAction := FarmerAndCabbage
+}
+
+action FarmerAlone {
+  require (goat_pos = wolf_pos → farmer_pos = goat_pos) ∧ (goat_pos = cabbage_pos → farmer_pos = goat_pos)
+  if farmer_pos = far then
+    farmer_pos := near
+  else
+    farmer_pos := far
+  -- lastAction := FarmerAlone
+}
+
+
+invariant [unsolved] ¬ (goat_pos = far ∧ wolf_pos = far ∧ cabbage_pos = far ∧ farmer_pos = far)
+
+#gen_spec
+
+
+#prepareExecution
+
+#finitizeTypes position
+
+
+def modelCheckerResult' := (runModelCheckerx initVeilMultiExecM nextVeilMultiExecM labelList (fun ρ σ => unsolved ρ σ) ((fun ρ σ => true)) {} hash).snd
+def statesJson : Lean.Json := Lean.toJson (recoverTrace initVeilMultiExecM nextVeilMultiExecM {} (collectTrace' modelCheckerResult'))
+open ProofWidgets
+open scoped ProofWidgets.Jsx
+#html <ModelCheckerView trace={statesJson} layout={"vertical"} />
+
+
+
+end RiverCrossing
