Test/Diehard_clear.lean
@@ -1,0 +1,120 @@
+import Veil
+import Veil.Frontend.DSL.Action.Extraction.Extract
+import Veil.Core.Tools.Checker.Concrete.Main
+import ProofWidgets.Component.HtmlDisplay
+
+veil module DieHard
+
+individual big : Nat
+-- individual tmp : Nat
+individual small : Nat
+
+#gen_state
+
+after_init {
+  big := 0
+  small := 0
+}
+
+
+action FillSmallJug {
+  -- (small : Nat) := 3
+  small := 3
+  big := big
+}
+
+
+action FillBigJug  {
+  big := 5
+  small := small
+}
+
+
+action EmptySmallJug {
+  -- (small : Nat) := 0
+  small := 0
+  big := big
+}
+
+
+action EmptyBigJug {
+  -- (big : Nat) := 0w
+  big := 0
+  small := small
+}
+
+
+action SmallToBig {
+  let tmp := big
+  big := if big + small < 5 then big + small else 5
+  small := small - (big - tmp)
+}
+
+
+
+action BigToSmall {
+  let tmp := small
+  small := if big + small < 3 then big + small else 3
+  big := big - (small - tmp)
+}
+
+
+invariant [typeOK] small≤ 3 ∧ big ≤ 5
+
+
+invariant [not_solved] big ≠ 4
+
+#gen_spec
+
+
+#time #check_invariants
+section
+
+
+veil_variables
+
+omit χ χ_rep χ_rep_lawful
+
+deriving_FinOrdToJson_Domain
+
+specify_FieldConcreteType
+
+deriving_BEq_FieldConcreteType
+
+deriving_Repr_FieldConcreteType
+
+deriving_Hashable_FieldConcreteType
+
+deriving_rep_FieldRepresentation
+
+deriving_lawful_FieldRepresentation
+
+deriving_Inhabited_State
+
+end
+
+gen_NextAct
+gen_executable_NextAct
+
+
+#Concretize
+
+deriving_BEqHashable_ConcreteState
+simple_deriving_repr_for' State
+deriving instance Repr for Label
+deriving instance Inhabited for Theory
+deriving_toJson_for_state
+deriving_DecidableProps_state
+
+
+def modelCheckerResult' := (runModelCheckerx initVeilMultiExecM nextVeilMultiExecM labelList (fun ρ σ => not_solved ρ σ) ((fun ρ σ => true)) {} hash).snd
+def statesJson : Lean.Json :=
+  Lean.toJson (recoverTrace initVeilMultiExecM nextVeilMultiExecM {} (collectTrace' modelCheckerResult'))
+
+open ProofWidgets
+open scoped ProofWidgets.Jsx
+#html <ModelCheckerView trace={statesJson} layout={"vertical"} />
+
+
+
+end DieHard
