Test/GooseFoxCabbage.lean
@@ -1,0 +1,194 @@
+import Veil
+import Veil.Frontend.DSL.Action.Extraction.Extract
+import Veil.Core.Tools.Checker.Concrete.Main
+import ProofWidgets.Component.HtmlDisplay
+
+veil module RiverCrossing
+
+enum position = {near, far}
+individual wolf_pos : position
+individual goat_pos : position
+individual cabbage_pos : position
+individual farmer_pos : position
+
+#print position_Enum
+-- enum act = {Init, FarmerAndWolf, FarmerAndGoat, FarmerAndCabbage, FarmerAlone}
+-- individual lastAction : act
+
+#gen_state
+
+/-
+Puzzle Rules:
+ * If goat and wolf are on the same bank p, the farmer must also be on p.
+ * If goat and cabbage are on the same bank p, the farmer must also be on p.
+-/
+ghost relation safety_constraint :=
+     (goat_pos = wolf_pos → farmer_pos = goat_pos) ∧
+     (goat_pos = cabbage_pos → farmer_pos = goat_pos)
+
+after_init {
+  wolf_pos := near
+  goat_pos := near
+  cabbage_pos := near
+  farmer_pos := near
+  -- lastAction := Init
+}
+
+action FarmerAndWolf {
+  require (goat_pos = wolf_pos → farmer_pos = goat_pos) ∧ (goat_pos = cabbage_pos → farmer_pos = goat_pos)
+  require farmer_pos = wolf_pos
+
+  if farmer_pos = far then
+    farmer_pos := near
+    wolf_pos := near
+  else
+    farmer_pos := far
+    wolf_pos := far
+  -- lastAction := FarmerAndWolf
+}
+
+action FarmerAndGoat {
+  require (goat_pos = wolf_pos → farmer_pos = goat_pos) ∧ (goat_pos = cabbage_pos → farmer_pos = goat_pos)
+  require farmer_pos = goat_pos
+  if farmer_pos = far then
+    farmer_pos := near
+    goat_pos := near
+  else
+    farmer_pos := far
+    goat_pos := far
+  -- lastAction := FarmerAndGoat
+}
+
+
+action FarmerAndCabbage {
+  require (goat_pos = wolf_pos → farmer_pos = goat_pos) ∧ (goat_pos = cabbage_pos → farmer_pos = goat_pos)
+  require farmer_pos = cabbage_pos
+  if farmer_pos = far then
+    farmer_pos := near
+    cabbage_pos := near
+  else
+    farmer_pos := far
+    cabbage_pos := far
+  -- lastAction := FarmerAndCabbage
+}
+
+action FarmerAlone {
+  require (goat_pos = wolf_pos → farmer_pos = goat_pos) ∧ (goat_pos = cabbage_pos → farmer_pos = goat_pos)
+  if farmer_pos = far then
+    farmer_pos := near
+  else
+    farmer_pos := far
+  -- lastAction := FarmerAlone
+}
+
+
+invariant [unsolved] ¬ (goat_pos = far ∧ wolf_pos = far ∧ cabbage_pos = far ∧ farmer_pos = far)
+
+#gen_spec
+
+-- section
+
+-- veil_variables
+
+-- omit χ χ_rep χ_rep_lawful
+
+open Veil Extract
+
+#check position
+
+-- deriving_FinOrdToJson_Domain
+-- specify_FieldConcreteType
+
+
+instance instFinEnumForToDomain (position : Type) [FinEnum position] (f : State.Label) :
+    (Veil.IteratedProd <| (List.map FinEnum <| (State.Label.toDomain position) f)) := by
+  cases f <;> infer_instance_for_iterated_prod
+instance instOrdForToDomain' (position : Type) [Ord position] (f : State.Label) :
+    (Ord (Veil.IteratedProd' <| (State.Label.toDomain position) f)) := by
+  cases f <;> dsimp only [Veil.IteratedProd', List.foldr, State.Label.toDomain, State.Label.toCodomain] <;>
+    infer_instance
+instance instToJsonForToDomain' (position : Type) [Lean.ToJson position] (f : State.Label) :
+    (Lean.ToJson (Veil.IteratedProd' <| (State.Label.toDomain position) f)) := by
+  cases f <;> dsimp only [Veil.IteratedProd', List.foldr, State.Label.toDomain, State.Label.toCodomain] <;>
+    infer_instance
+instance instToJsonForToCodomain [Lean.ToJson position] (f : State.Label) :
+    (Lean.ToJson ((State.Label.toCodomain position) f)) := by
+  cases f <;> dsimp only [Veil.IteratedProd', List.foldr, State.Label.toDomain, State.Label.toCodomain] <;>
+    infer_instance
+
+
+abbrev FieldConcreteType (position : Type) [Ord position] (f : State.Label) : Type :=
+  match f with
+  | State.Label.wolf_pos => (State.Label.toCodomain position) State.Label.wolf_pos
+  | State.Label.goat_pos => (State.Label.toCodomain position) State.Label.goat_pos
+  | State.Label.cabbage_pos => (State.Label.toCodomain position) State.Label.cabbage_pos
+  | State.Label.farmer_pos => (State.Label.toCodomain position) State.Label.farmer_pos
+
+#check FieldConcreteType
+
+instance
+{ρ σ position : Type}
+[position_dec_eq : DecidableEq position]
+[position_inhabited : Inhabited position]
+[position_isEnum : position_Enum position]
+-- (χ : State.Label → Type)
+-- [χ_rep : (f : State.Label) → FieldRepresentation (State.Label.toDomain position f) (State.Label.toCodomain position f) (χ f)]
+-- [χ_rep_lawful : ∀ (f : State.Label), LawfulFieldRepresentation (State.Label.toDomain position f) (State.Label.toCodomain position f) (χ f) (χ_rep f)]
+-- [σ_sub : IsSubStateOf (State position χ) σ]
+-- [ρ_sub : IsSubReaderOf (Theory position) ρ]
+[Ord position]:
+    (BEq (FieldConcreteType position State.Label.wolf_pos)) :=
+  by
+  dsimp only [FieldConcreteType, Veil.IteratedProd', State.Label.toDomain, State.Label.toCodomain]
+  repeat'
+    (first
+      | infer_instance
+      | constructor)
+
+
+#exit
+deriving_BEq_FieldConcreteType
+
+deriving_Hashable_FieldConcreteType
+
+deriving_rep_FieldRepresentation
+
+deriving_lawful_FieldRepresentation
+
+deriving_Inhabited_State
+
+deriving_Decidable_Props
+
+
+gen_NextAct
+
+gen_executable_NextAct
+
+deriving_Enum_Insts
+-- deriving_enum_instance_for position
+-- deriving_ord_hashable_for_enum position
+-- deriving_propCmp_for_enum position
+
+#Concretize position
+
+
+deriving_BEqHashable_ConcreteState
+simple_deriving_repr_for' State
+deriving instance Repr for Label
+deriving instance Inhabited for Theory
+deriving_toJson_for_state
+deriving_DecidableProps_state
+
+
+def modelCheckerResult' := (runModelCheckerx initVeilMultiExecM nextVeilMultiExecM labelList (fun ρ σ => unsolved ρ σ) ((fun ρ σ => true)) {} hash).snd
+
+
+def statesJson : Lean.Json :=
+  Lean.toJson (recoverTrace initVeilMultiExecM nextVeilMultiExecM {} (collectTrace' modelCheckerResult'))
+open ProofWidgets
+open scoped ProofWidgets.Jsx
+#html <ModelCheckerView trace={statesJson} layout={"vertical"} />
+
+
+
+end RiverCrossing
