Test/structure.lean
@@ -1,0 +1,1036 @@
+import Veil
+import Veil.Frontend.DSL.Action.Extraction.Extract
+import Veil.Core.Tools.Checker.Concrete.Main
+-- ----- MODULE 0_mutex -----
+veil module Mutex
+
+-- \* BEGIN TRANSLATION (chksum(pcal) = "b0b421b7" /\ chksum(tla) = "c2205e03")
+-- VARIABLES
+-- 1. locked,
+-- 2. wait_queue_num_wakers,
+-- 3. wait_queue_wakers,
+-- 4. has_woken,
+-- 5. pc,
+-- 6. stack,
+-- 7. waker
+--
+type process
+-- type seq_t
+individual locked : Bool
+enum states = { pre_check_lock, wait_until, enqueue_waker,
+                check_lock, check_has_woken,
+                release_lock, wake_one, wake_one_loop,
+                wake_up, start, cs, Done }
+
+-- instantiate seq : TotalOrderWithZero seq_t
+-- immutable individual one : seq_t
+-- individual wait_queue_num_wakers : seq_t
+
+individual wait_queue_wakers : List process
+
+relation has_woken (th: process)
+relation pc (self: process) (st: states)
+immutable individual none : process
+
+/-
+Decompose the structure into two relations:
+- `stack_pc` : process → seq_t → states
+- `stack_waker` : process → seq_t → process.
+
+To model the list, we use two individuals, which represent
+the head and tail of the list respectively.
+
+[ procedure |->  "unlock",
+  pc        |->  "Done",
+  waker     |->  waker[self] ]
+-/
+
+structure Cell (states process : Type) where
+  pc : states
+  waker : process
+deriving DecidableEq, Inhabited, BEq, Hashable, Ord, Repr, Lean.ToJson
+
+function stack : process → List (Cell states process)
+relation waker (self: process) (waker: process)
+
+#gen_state
+-- theory ghost relation lt (x y : seq_t) := (seq.le x y ∧ x ≠ y)
+-- theory ghost relation next (x y : seq_t) := (lt x y ∧ ∀ z, lt x z → seq.le y z)
+-- vars == << locked, wait_queue_num_wakers, wait_queue_wakers, has_woken, pc,
+--            stack, waker >>
+
+-- ProcSet == (Procs)
+
+-- Init == (* Global variables *)
+--         /\ locked = FALSE
+--         /\ wait_queue_num_wakers = 0
+--         /\ wait_queue_wakers = <<>>
+--         /\ has_woken = [x \in Procs |-> FALSE]
+--         (* Procedure unlock *)
+--         /\ waker = [ self \in ProcSet |-> NONE]
+--         /\ stack = [self \in ProcSet |-> << >>]
+--         /\ pc = [self \in ProcSet |-> "start"]
+
+after_init {
+  locked := false
+
+  wait_queue_wakers := []
+  has_woken P := false
+  waker P W := W == none
+
+  -- stack_pc P := []
+  -- stack_waker P := []
+  stack P := []
+  pc P S := S == start
+}
+
+-- start(self) == /\ pc[self] = "start"
+--                /\ stack' = [stack EXCEPT ![self] = << [ procedure |->  "lock",
+--                                                         pc        |->  "cs" ] >>
+--                                                     \o stack[self]]
+--                /\ pc' = [pc EXCEPT ![self] = "pre_check_lock"]
+--                /\ UNCHANGED << locked, wait_queue_num_wakers,
+--                                wait_queue_wakers, has_woken, waker >>
+action _start (self : process) {
+  require pc self start
+  -- let t := stack_pc self
+  -- stack_pc self := cs :: (stack_pc self)
+  let random_waker ← pick process
+  -- stack_waker self := random_waker :: (stack_waker self)
+  stack self := { pc := cs, waker := random_waker } :: (stack self)
+  pc self S := S == pre_check_lock
+}
+
+
+-- pre_check_lock(self) == /\ pc[self] = "pre_check_lock"
+--                         /\ IF locked = FALSE
+--                               THEN /\ locked' = TRUE
+--                                    /\ pc' = [pc EXCEPT ![self] = Head(stack[self]).pc]
+--                                    /\ stack' = [stack EXCEPT ![self] = Tail(stack[self])]
+--                               ELSE /\ pc' = [pc EXCEPT ![self] = "wait_until"]
+--                                    /\ UNCHANGED << locked, stack >>
+--                         /\ UNCHANGED << wait_queue_num_wakers,
+--                                         wait_queue_wakers, has_woken, waker >>
+action _pre_check_lock (self : process) {
+  require pc self pre_check_lock
+  if locked == false then
+    locked := true
+    -- assert stack self ≠ []
+    let head_stack_pc_state := (stack self).head!.pc
+    pc self S := S == head_stack_pc_state
+    stack self := (stack self).tail
+  else
+    pc self S := S == wait_until
+}
+
+-- wait_until(self) == /\ pc[self] = "wait_until"
+--                     /\ pc' = [pc EXCEPT ![self] = "enqueue_waker"]
+--                     /\ UNCHANGED << locked, wait_queue_num_wakers,
+--                                     wait_queue_wakers, has_woken, stack, waker >>
+action _wait_until (self : process) {
+  require pc self wait_until
+  pc self S := S == enqueue_waker
+}
+
+-- enqueue_waker(self) == /\ pc[self] = "enqueue_waker"
+--                        /\ wait_queue_num_wakers' = wait_queue_num_wakers + 1
+--                        /\ wait_queue_wakers' = Append(wait_queue_wakers, self)
+--                        /\ pc' = [pc EXCEPT ![self] = "check_lock"]
+--                        /\ UNCHANGED << locked, has_woken, stack, waker >>
+action _enqueue_waker (self : process) {
+  require pc self enqueue_waker
+  wait_queue_wakers := wait_queue_wakers.append [self]
+  pc self S := S == check_lock
+}
+
+
+-- check_lock(self) == /\ pc[self] = "check_lock"
+--                     /\ IF locked = FALSE
+--                           THEN /\ locked' = TRUE
+--                                /\ pc' = [pc EXCEPT ![self] = Head(stack[self]).pc]
+--                                /\ stack' = [stack EXCEPT ![self] = Tail(stack[self])]
+--                           ELSE /\ pc' = [pc EXCEPT ![self] = "check_has_woken"]
+--                                /\ UNCHANGED << locked, stack >>
+--                     /\ UNCHANGED << wait_queue_num_wakers, wait_queue_wakers,
+--                                     has_woken, waker >>
+action _check_lock (self : process) {
+  require pc self check_lock
+  if locked == false then
+    locked := true
+    -- assert stack self ≠ []
+    let head_stack_pc_state := (stack self).head!.pc
+    pc self S := S == head_stack_pc_state
+    stack self := (stack self).tail
+  else
+    pc self S := S == check_has_woken
+}
+
+-- check_has_woken(self) == /\ pc[self] = "check_has_woken"
+--                          /\ has_woken[self]
+--                          /\ has_woken' = [has_woken EXCEPT ![self] = FALSE]
+--                          /\ pc' = [pc EXCEPT ![self] = "wait_until"]
+--                          /\ UNCHANGED << locked, wait_queue_num_wakers,
+--                                          wait_queue_wakers, stack, waker >>
+action check_has_woken (self : process) {
+  require pc self check_has_woken
+  require has_woken self
+  has_woken self := false
+  pc self S := S == wait_until
+}
+
+-- lock(self) == pre_check_lock(self) \/ wait_until(self)
+--                  \/ enqueue_waker(self) \/ check_lock(self)
+--                  \/ check_has_woken(self)
+
+
+-- release_lock(self) == /\ pc[self] = "release_lock"
+--                       /\ locked' = FALSE
+--                       /\ pc' = [pc EXCEPT ![self] = "wake_one"]
+--                       /\ UNCHANGED << wait_queue_num_wakers, wait_queue_wakers,
+--                                       has_woken, stack, waker >>
+action _release_lock (self : process) {
+  require pc self release_lock
+  locked := false
+  pc self S := S == wake_one
+}
+
+
+-- wake_one(self) == /\ pc[self] = "wake_one"
+--                   /\ IF wait_queue_num_wakers = 0
+--                         THEN /\ pc' = [pc EXCEPT ![self] = Head(stack[self]).pc]
+--                              /\ waker' = [waker EXCEPT ![self] = Head(stack[self]).waker]
+--                              /\ stack' = [stack EXCEPT ![self] = Tail(stack[self])]
+--                         ELSE /\ pc' = [pc EXCEPT ![self] = "wake_one_loop"]
+--                              /\ UNCHANGED << stack, waker >>
+--                   /\ UNCHANGED << locked, wait_queue_num_wakers,
+--                                   wait_queue_wakers, has_woken >>
+action _wake_one (self : process) {
+  require pc self wake_one
+  if wait_queue_wakers.length == 0 then
+    -- assert stack self ≠ []
+    let head_stack_pc_state := (stack self).head!.pc
+    pc self S := S == head_stack_pc_state
+    let headwaker_stack_waker := (stack self).head!.waker
+    waker self W := W == headwaker_stack_waker
+    stack self := (stack self).tail
+  else
+    pc self S := S == wake_one_loop
+}
+
+-- wake_one_loop(self) == /\ pc[self] = "wake_one_loop"
+--                        /\ IF Len(wait_queue_wakers) /= 0
+--                              THEN /\ waker' = [waker EXCEPT ![self] = Head(wait_queue_wakers)]
+--                                   /\ wait_queue_wakers' = Tail(wait_queue_wakers)
+--                                   /\ wait_queue_num_wakers' = wait_queue_num_wakers - 1
+--                                   /\ pc' = [pc EXCEPT ![self] = "wake_up"]
+--                                   /\ stack' = stack
+--                              ELSE /\ pc' = [pc EXCEPT ![self] = Head(stack[self]).pc]
+--                                   /\ waker' = [waker EXCEPT ![self] = Head(stack[self]).waker]
+--                                   /\ stack' = [stack EXCEPT ![self] = Tail(stack[self])]
+--                                   /\ UNCHANGED << wait_queue_num_wakers,
+--                                                   wait_queue_wakers >>
+--                        /\ UNCHANGED << locked, has_woken >>
+
+action _wake_one_loop (self : process) {
+  require pc self wake_one_loop
+  if wait_queue_wakers.length != 0 then
+    let head_waker := wait_queue_wakers.head!
+    waker self W := W == head_waker
+    wait_queue_wakers := wait_queue_wakers.tail
+    pc self S := S == wake_up
+  else
+    let head_stack_pc_state := (stack self).head!.pc
+    pc self S := S == head_stack_pc_state
+    -- stack self := (stack self).tail
+
+    let headwaker_stack_waker := (stack self).head!.waker
+    waker self W := W == headwaker_stack_waker
+    stack self := (stack self).tail
+}
+
+
+-- wake_up(self) == /\ pc[self] = "wake_up"
+--                  /\ IF has_woken[waker[self]] = FALSE
+--                        THEN /\ has_woken' = [has_woken EXCEPT ![waker[self]] = TRUE]
+--                             /\ pc' = [pc EXCEPT ![self] = Head(stack[self]).pc]
+--                             /\ waker' = [waker EXCEPT ![self] = Head(stack[self]).waker]
+--                             /\ stack' = [stack EXCEPT ![self] = Tail(stack[self])]
+--                        ELSE /\ pc' = [pc EXCEPT ![self] = "wake_one_loop"]
+--                             /\ UNCHANGED << has_woken, stack, waker >>
+--                  /\ UNCHANGED << locked, wait_queue_num_wakers,
+--                                  wait_queue_wakers >>
+action _wake_up (self : process) {
+  require pc self wake_up
+
+  if ∃t, waker self t then
+    let waker_self :| waker self waker_self
+
+    /- Condition 1: -/
+    if has_woken waker_self == false then
+      has_woken waker_self := true
+      let head_stack_pc_state := (stack self).head!.pc
+      pc self S := S == head_stack_pc_state
+
+      let headwaker_stack_waker := (stack self).head!.waker
+      waker self W := W == headwaker_stack_waker
+
+      stack self := (stack self).tail
+    else
+      pc self S := S == wake_one_loop
+
+  -- else
+  --   /- Exception handle -/
+  --   let waker_self := none
+  --   if has_woken waker_self == false then
+  --     has_woken waker_self := true
+  --     let head_stack_pc_state := (stack_pc self).head!
+  --     pc self S := S == head_stack_pc_state
+  --     stack_pc self := (stack_pc self).tail
+
+  --     let headwaker_stack_waker := (stack_waker self).head!
+  --     waker self W := W == headwaker_stack_waker
+  --     stack_waker self := (stack_waker self).tail
+  --   else
+  --     pc self S := S == wake_one_loop
+
+}
+
+
+-- unlock(self) == release_lock(self) \/ wake_one(self) \/ wake_one_loop(self)
+--                    \/ wake_up(self)
+
+
+-- cs(self) == /\ pc[self] = "cs"
+--             /\ TRUE
+--             /\ stack' = [stack EXCEPT ![self] = << [ procedure |->  "unlock",
+--                                                      pc        |->  "Done",
+--                                                      waker     |->  waker[self] ] >>
+--                                                  \o stack[self]]
+--             /\ waker' = [waker EXCEPT ![self] = NONE]
+--             /\ pc' = [pc EXCEPT ![self] = "release_lock"]
+--             /\ UNCHANGED << locked, wait_queue_num_wakers, wait_queue_wakers,
+--                             has_woken >>
+action _cs(self : process) {
+  require pc self cs
+  -- stack_pc self := Done :: (stack_pc self)
+  if ∃t, waker self t then
+    let waker_self :| waker self waker_self
+    -- stack_waker self := waker_self :: (stack_waker self)
+    -- waker self W := false
+    waker self W := W == none
+    stack self := { pc := Done, waker := waker_self } :: (stack self)
+  -- else
+  --   let waker_self := none
+  --   stack_waker self := waker_self :: (stack_waker self)
+  --   waker self W := W == none
+
+  pc self S := S == release_lock
+}
+
+termination [allDone] pc S Done
+invariant [mutual_exclusion] ∀ I J, I ≠ J → ¬ (pc I cs ∧ pc J cs)
+
+
+#gen_spec
+
+-- open Lean Meta Elab Command Veil in
+-- scoped elab "⌞? " t:term " ⌟" : term => do
+--   let lenv ← localEnv.get
+--   let some mod := lenv.currentModule | throwError s!"Not in a module"
+--   Term.elabTerm (← `(term| $t $(← mod.sortIdents)*)) none
+
+-- -- #time #check_invariants
+
+-- section
+
+-- veil_variables
+
+
+-- omit χ χ_rep χ_rep_lawful
+
+-- open Veil Extract
+
+
+-- variable [FinEnum process] [Hashable process] [Ord process]
+-- variable [FinEnum states] [Hashable states] [Ord states]
+-- -- variable [FinEnum Cell] [Hashable Cell] [Ord Cell]
+-- variable [Std.LawfulEqCmp (Ord.compare (self := inferInstanceAs (Ord process)))]
+-- variable [Std.TransCmp (Ord.compare (self := inferInstanceAs (Ord process)))]
+
+-- variable [Std.LawfulEqCmp (Ord.compare (self := inferInstanceAs (Ord states)))]
+-- variable [Std.TransCmp (Ord.compare (self := inferInstanceAs (Ord states)))]
+
+-- variable [Ord (process × states)]
+-- variable [Std.LawfulEqCmp (Ord.compare (self := inferInstanceAs (Ord (process × states))))]
+-- variable [Std.TransCmp (Ord.compare (self := inferInstanceAs (Ord (process × states))))]
+
+-- variable [Ord (process × process)]
+-- variable [Std.LawfulEqCmp (Ord.compare (self := inferInstanceAs (Ord (process × process))))]
+-- variable [Std.TransCmp (Ord.compare (self := inferInstanceAs (Ord (process × process))))]
+
+-- -- variable [Ord (process × List Cell)]
+-- -- variable [Std.LawfulEqCmp (Ord.compare (self := inferInstanceAs (Ord (process × List Cell))))]
+-- -- variable [Std.TransCmp (Ord.compare (self := inferInstanceAs (Ord (process × List Cell))))]
+
+
+-- #print State.Label.toDomain
+
+-- -- example (f : State.Label) : (⌞? State.Label.toDomain ⌟) f = [ℕ]:= by
+-- --   unfold State.Label.toDomain
+
+-- -- example (f : State.Label) : ((⌞? State.Label.toCodomain ⌟) f) = ℕ := by
+-- --   unfold State.Label.toCodomain
+-- --   simp
+
+-- def instFinEnumForComponents (f : State.Label)
+--   : (IteratedProd <| List.map FinEnum <| (⌞? State.Label.toDomain ⌟) f) := by
+--   cases f <;>
+--     infer_instance_for_iterated_prod
+
+-- instance instFinEnumForCodomain [FinEnum (List (Cell states process))][FinEnum (List process)] (f : State.Label)
+--   : (FinEnum ((⌞? State.Label.toCodomain ⌟) f)) := by
+--   cases f <;>
+--     dsimp only [IteratedProd, List.foldr, State.Label.toCodomain, State.Label.toCtorIdx] <;>
+--     infer_instance
+
+-- instance instFinEnumForComponents' (f : State.Label)
+--   : FinEnum (IteratedProd' <| (⌞? State.Label.toDomain ⌟) f) := by
+--   cases f <;>
+--     dsimp only [IteratedProd', List.foldr, State.Label.toDomain] <;>
+--     infer_instance
+
+-- instance instDecidableEqForComponents' (f : State.Label)
+--   : DecidableEq (IteratedProd <| (⌞? State.Label.toDomain ⌟) f) := by
+--   cases f <;>
+--     dsimp only [IteratedProd, List.foldr, State.Label.toDomain] <;>
+--     infer_instance
+
+-- instance instDecidableEqForComponents'' (f : State.Label)
+--   : DecidableEq (IteratedProd' <| (⌞? State.Label.toDomain ⌟) f) := by
+--   cases f <;>
+--     dsimp only [IteratedProd', State.Label.toDomain] <;>
+--     infer_instance
+
+-- instance instHashableForComponents (f : State.Label)
+--   : Hashable (IteratedProd <| (⌞? State.Label.toDomain ⌟) f) := by
+--   cases f <;>
+--     dsimp only [IteratedProd, List.foldr, State.Label.toDomain] <;>
+--     infer_instance
+
+-- instance instHashableForComponents' (f : State.Label)
+--   : Hashable (IteratedProd' <| (⌞? State.Label.toDomain ⌟) f) := by
+--   cases f <;>
+--     dsimp only [IteratedProd', State.Label.toDomain] <;>
+--     infer_instance
+
+
+-- instance [Ord α] [Ord β] : Ord (α × β) where
+--   compare x y := match x, y with
+--     | (a, b), (a', b') => compare a a' |>.then (compare b b')
+
+-- instance instOrderForComponents' (f : State.Label)
+--   : Ord (IteratedProd' <| (⌞? State.Label.toDomain ⌟) f) := by
+--   cases f <;>
+--     dsimp only [IteratedProd', State.Label.toDomain] <;>
+--     infer_instance
+
+
+-- instance (f : State.Label) : Ord (IteratedProd' (State.Label.toDomain process states f)) := by
+--   cases f <;>
+--     dsimp only [IteratedProd', State.Label.toDomain, State.Label.toCodomain] <;>
+--     infer_instance
+
+
+-- abbrev FieldConcreteType (f : State.Label) : Type :=
+--   match f with
+--   | State.Label.locked =>
+--     ((⌞? State.Label.toCodomain ⌟) State.Label.locked)
+--   | State.Label.wait_queue_wakers =>
+--     ((⌞? State.Label.toCodomain ⌟) State.Label.wait_queue_wakers)
+--   | State.Label.has_woken =>
+--     Std.TreeSet (IteratedProd' <| (⌞? State.Label.toDomain ⌟) State.Label.has_woken)
+--   | State.Label.pc =>
+--     Std.TreeSet (IteratedProd' <| (⌞? State.Label.toDomain ⌟) State.Label.pc)
+--   /- `stack_pc` is a `function` field -/
+--   | State.Label.stack =>
+--     -- Std.TreeSet (IteratedProd' <| (⌞? State.Label.toDomain ⌟) State.Label.stack_pc)
+--     -- Std.TreeSet (process × List process)
+--     TotalTreeMap (IteratedProd' <| (⌞? State.Label.toDomain ⌟) State.Label.stack)
+--     ((⌞? State.Label.toCodomain ⌟) State.Label.stack)
+--   /- `stack_stack` is a `function` field -/
+--   /- `stack_` is a `relation` -/
+--   | State.Label.waker =>
+--     Std.TreeSet (IteratedProd' <| (⌞? State.Label.toDomain ⌟) State.Label.waker)
+
+
+-- instance instReprForComponents [Repr process] [Repr states] [Repr (TotalTreeMap process (List (Cell states process)) compare)] (f : State.Label)
+--   : Repr ((⌞? FieldConcreteType ⌟) f) := by
+--   cases f <;>
+--     dsimp only [IteratedProd', FieldConcreteType, State.Label.toDomain, State.Label.toCodomain] <;>
+--     infer_instance
+
+
+-- instance : Inhabited ((⌞? State ⌟) (⌞? FieldConcreteType ⌟)) := by
+--   constructor ; constructor <;>
+--   dsimp only [FieldConcreteType, State.Label.toCodomain] <;>
+--   -- exact default
+--   -- infer_instance_for_iterated_prod
+--   try exact default
+--   -- set_option trace.Meta.synthInstance.answer true in
+--   -- apply instInhabitedTotalTreeMapOfFinEnumOfLawfulEqCmpOfTransCmpOfDecidableEq.default
+
+
+
+-- open TotalMapLike
+-- #check instTotalMapLikeAsFieldRep
+-- instance rep (f : State.Label) : FieldRepresentation
+--   ((⌞? State.Label.toDomain ⌟) f)
+--   ((⌞? State.Label.toCodomain ⌟) f)
+--   ((⌞? FieldConcreteType ⌟) f) :=
+--   -- by cases f <;> apply instFinsetLikeAsFieldRep <;> apply instFinEnumForComponents
+--   match f with
+--   | State.Label.locked => by
+--       dsimp only [FieldConcreteType, State.Label.toCodomain, State.Label.toDomain] ;
+--       infer_instance
+--   | State.Label.wait_queue_wakers =>by
+--       dsimp only [FieldConcreteType, State.Label.toCodomain, State.Label.toDomain] ;
+--       infer_instance
+--   | State.Label.has_woken =>
+--     instFinsetLikeAsFieldRep (IteratedProd'.equiv) ((⌞? instFinEnumForComponents ⌟) State.Label.has_woken)
+--   | State.Label.pc =>
+--     instFinsetLikeAsFieldRep (IteratedProd'.equiv) ((⌞? instFinEnumForComponents ⌟) State.Label.pc)
+--   | State.Label.stack =>
+--     instTotalMapLikeAsFieldRep (IteratedProd'.equiv) ((⌞? instFinEnumForComponents ⌟) State.Label.stack)
+--   | State.Label.waker =>
+--     instFinsetLikeAsFieldRep (IteratedProd'.equiv) ((⌞? instFinEnumForComponents ⌟) State.Label.waker)
+
+-- #check instTotalMapLikeAsFieldRep
+
+-- instance lawful (f : State.Label): LawfulFieldRepresentation
+--   ((⌞? State.Label.toDomain ⌟) f)
+--   ((⌞? State.Label.toCodomain ⌟) f)
+--   ((⌞? FieldConcreteType ⌟) f)
+--   ((⌞? rep ⌟) f) :=-- by cases f <;> apply instFinsetLikeAsFieldRep <;> apply instFinEnumForComponents
+--   match f with
+--   | State.Label.locked => by
+--       dsimp only [FieldConcreteType, State.Label.toCodomain, State.Label.toDomain, rep, id]
+--       infer_instance
+--   | State.Label.wait_queue_wakers => by
+--       dsimp only [FieldConcreteType, State.Label.toCodomain, State.Label.toDomain, rep, id]
+--       infer_instance
+--   | State.Label.has_woken =>
+--     instFinsetLikeLawfulFieldRep (IteratedProd'.equiv) ((⌞? instFinEnumForComponents ⌟) State.Label.has_woken)
+--   | State.Label.pc =>
+--     instFinsetLikeLawfulFieldRep (IteratedProd'.equiv) ((⌞? instFinEnumForComponents ⌟) State.Label.pc)
+--   | State.Label.stack =>by
+--       dsimp only [FieldConcreteType, State.Label.toCodomain, State.Label.toDomain, rep, id]
+--       infer_instance
+--   | State.Label.waker =>
+--     instFinsetLikeLawfulFieldRep (IteratedProd'.equiv) ((⌞? instFinEnumForComponents ⌟) State.Label.waker)
+-- end
+
+-- attribute [local dsimpFieldRepresentationGet, local dsimpFieldRepresentationSet]
+--   instFinEnumForComponents in
+-- -- attribute [local dsimpFieldRepresentationGet] FourNodes.equiv_IteratedProd in
+-- #specialize_nextact with FieldConcreteType
+--   injection_begin
+--     -- [FinEnum process] [Hashable process] [Ord process]
+--     -- [FinEnum states] [Hashable states] [Ord states]
+--     -- [Std.LawfulEqCmp (Ord.compare (self := inferInstanceAs (Ord process)))]
+--     -- [Std.TransCmp (Ord.compare (self := inferInstanceAs (Ord process)))]
+--     -- [Std.LawfulEqCmp (Ord.compare (self := inferInstanceAs (Ord states)))]
+--     -- [Std.TransCmp (Ord.compare (self := inferInstanceAs (Ord states)))]
+
+--     -- [Ord (process × states)]
+--     -- [Std.LawfulEqCmp (Ord.compare (self := inferInstanceAs (Ord (process × states))))]
+--     -- [Std.TransCmp (Ord.compare (self := inferInstanceAs (Ord (process × states))))]
+
+--     -- [Ord (process × process)]
+--     -- [Std.LawfulEqCmp (Ord.compare (self := inferInstanceAs (Ord (process × process))))]
+--     -- [Std.TransCmp (Ord.compare (self := inferInstanceAs (Ord (process × process))))]
+--     [FinEnum process] [Hashable process] [Ord process]
+--     [FinEnum states] [Hashable states] [Ord states]
+--     [Std.LawfulEqCmp (Ord.compare (self := inferInstanceAs (Ord process)))]
+--     [Std.TransCmp (Ord.compare (self := inferInstanceAs (Ord process)))]
+--     [Std.LawfulEqCmp (Ord.compare (self := inferInstanceAs (Ord states)))]
+--     [Std.TransCmp (Ord.compare (self := inferInstanceAs (Ord states)))]
+
+--     [Ord (process × states)]
+--     [Std.LawfulEqCmp (Ord.compare (self := inferInstanceAs (Ord (process × states))))]
+--     [Std.TransCmp (Ord.compare (self := inferInstanceAs (Ord (process × states))))]
+
+--     [Ord (process × process)]
+--     [Std.LawfulEqCmp (Ord.compare (self := inferInstanceAs (Ord (process × process))))]
+--     [Std.TransCmp (Ord.compare (self := inferInstanceAs (Ord (process × process))))]
+--   injection_end => NextAct'
+
+
+
+-- #gen_executable_list! log_entry_being Std.Format
+--   targeting NextAct'
+--   injection_begin
+--     [FinEnum process] [Hashable process] [Ord process]
+--     [FinEnum states] [Hashable states] [Ord states]
+--     [Std.LawfulEqCmp (Ord.compare (self := inferInstanceAs (Ord process)))]
+--     [Std.TransCmp (Ord.compare (self := inferInstanceAs (Ord process)))]
+--     [Std.LawfulEqCmp (Ord.compare (self := inferInstanceAs (Ord states)))]
+--     [Std.TransCmp (Ord.compare (self := inferInstanceAs (Ord states)))]
+
+--     [Ord (process × states)]
+--     [Std.LawfulEqCmp (Ord.compare (self := inferInstanceAs (Ord (process × states))))]
+--     [Std.TransCmp (Ord.compare (self := inferInstanceAs (Ord (process × states))))]
+
+--     [Ord (process × process)]
+--     [Std.LawfulEqCmp (Ord.compare (self := inferInstanceAs (Ord (process × process))))]
+--     [Std.TransCmp (Ord.compare (self := inferInstanceAs (Ord (process × process))))]
+--   injection_end
+
+#gen_spec
+
+
+deriving_FinOrdToJson_Domain
+
+specify_FieldConcreteType
+
+deriving_BEq_FieldConcreteType
+
+deriving_Hashable_FieldConcreteType
+
+deriving_rep_FieldRepresentation
+
+deriving_lawful_FieldRepresentation
+
+
+set_option pp.explicit true in
+set_option pp.instances true in
+#print instLawfulFieldRepForFieldRepresentation
+
+/- I'm confused about what's the `minimal instance` set needed to derive this instance. -/
+-- instance instLawfulFieldRepForFieldRepresentation [FinEnum process] [FinEnum states] [Ord process] [Ord states]
+--     [Std.LawfulEqCmp (Ord.compare (self := inferInstanceAs (Ord process)))]
+--     [Std.LawfulEqCmp (Ord.compare (self := inferInstanceAs (Ord states)))]
+--     [Std.TransCmp (Ord.compare (self := inferInstanceAs (Ord process)))]
+--     [Std.TransCmp (Ord.compare (self := inferInstanceAs (Ord states)))]
+--     -- [Std.LawfulEqCmp (Ord.compare (self := inferInstanceAs (Ord (Bool))))]
+--     -- [Std.TransCmp (Ord.compare (self := inferInstanceAs (Ord (Bool))))]
+--     -- [Std.LawfulEqCmp (Ord.compare (self := inferInstanceAs (Ord (List process))))]
+--     -- [Std.TransCmp (Ord.compare (self := inferInstanceAs (Ord (List process))))]
+--     [Std.LawfulEqCmp (Ord.compare (self := inferInstanceAs (Ord (process))))]
+--     [Std.TransCmp (Ord.compare (self := inferInstanceAs (Ord (process))))]
+--     [Std.LawfulEqCmp (Ord.compare (self := inferInstanceAs (Ord (process × (states)))))]
+--     [Std.TransCmp (Ord.compare (self := inferInstanceAs (Ord (process × (states)))))]
+--     -- [Std.LawfulEqCmp (Ord.compare (self := inferInstanceAs (Ord (process × (List (Cell states process))))))]
+--     -- [Std.TransCmp (Ord.compare (self := inferInstanceAs (Ord (process × (List (Cell states process))))))]
+--     [Std.LawfulEqCmp (Ord.compare (self := inferInstanceAs (Ord (process × (process)))))]
+--     [Std.TransCmp (Ord.compare (self := inferInstanceAs (Ord (process × (process)))))]
+--     (f : State.Label) :
+--     Veil.LawfulFieldRepresentation ((State.Label.toDomain process states) f) ((State.Label.toCodomain process states) f)
+--       ((FieldConcreteType process states) f) ((instRepForFieldRepresentation process states) f) :=
+--   by
+--   cases f <;>
+--     first
+--     |
+--       (dsimp only [FieldConcreteType,  State.Label.toCodomain,State.Label.toDomain, instRepForFieldRepresentation,
+--           Veil.IteratedProd', id];
+--         infer_instance)
+--     | (exact Veil.instFinsetLikeLawfulFieldRep Veil.IteratedProd'.equiv ((instFinEnumForToDomain process states) _))
+
+deriving_Inhabited_State
+
+
+theorem Mutex.instLawfulFieldRepForFieldRepresentation : ∀ {process states : Type} [inst : FinEnum process]
+  [inst_1 : FinEnum states] [inst_2 : Ord process] [inst_3 : Ord states]
+  [inst_4 : @Std.LawfulEqCmp process (@compare process (@inferInstanceAs (Ord process) inst_2))]
+  [inst_5 : @Std.LawfulEqCmp states (@compare states (@inferInstanceAs (Ord states) inst_3))]
+  [inst_6 : @Std.TransCmp process (@compare process (@inferInstanceAs (Ord process) inst_2))]
+  [inst_7 : @Std.TransCmp states (@compare states (@inferInstanceAs (Ord states) inst_3))] (f : State.Label),
+  Veil.LawfulFieldRepresentation (State.Label.toDomain process states f) (State.Label.toCodomain process states f)
+    (@FieldConcreteType process states inst_2 inst_3 f)
+    (@instRepForFieldRepresentation process states inst inst_1 inst_2 inst_3 inst_4 inst_5 inst_6 inst_7 f) :=
+fun {process states} [inst : FinEnum process] [inst_1 : FinEnum states] [inst_2 : Ord process] [inst_3 : Ord states]
+    [inst_4 : @Std.LawfulEqCmp process (@compare process (@inferInstanceAs (Ord process) inst_2))]
+    [inst_5 : @Std.LawfulEqCmp states (@compare states (@inferInstanceAs (Ord states) inst_3))]
+    [inst_6 : @Std.TransCmp process (@compare process (@inferInstanceAs (Ord process) inst_2))]
+    [inst_7 : @Std.TransCmp states (@compare states (@inferInstanceAs (Ord states) inst_3))] f =>
+  @State.Label.casesOn
+    (fun t =>
+      @Eq State.Label f t →
+        Veil.LawfulFieldRepresentation (State.Label.toDomain process states f) (State.Label.toCodomain process states f)
+          (@FieldConcreteType process states inst_2 inst_3 f)
+          (@instRepForFieldRepresentation process states inst inst_1 inst_2 inst_3 inst_4 inst_5 inst_6 inst_7 f))
+    f
+    (fun h =>
+      @Eq.ndrec State.Label State.Label.locked
+        (fun f =>
+          Veil.LawfulFieldRepresentation (State.Label.toDomain process states f)
+            (State.Label.toCodomain process states f) (@FieldConcreteType process states inst_2 inst_3 f)
+            (@instRepForFieldRepresentation process states inst inst_1 inst_2 inst_3 inst_4 inst_5 inst_6 inst_7 f))
+        (@id
+          (Veil.LawfulFieldRepresentation (State.Label.toDomain process states State.Label.locked)
+            (State.Label.toCodomain process states State.Label.locked)
+            (@FieldConcreteType process states inst_2 inst_3 State.Label.locked)
+            (@instRepForFieldRepresentation process states inst inst_1 inst_2 inst_3 inst_4 inst_5 inst_6 inst_7
+              State.Label.locked))
+          (@inferInstance
+            (Veil.LawfulFieldRepresentation (@List.nil Type) Bool Bool
+              (@inferInstance (Veil.FieldRepresentation (@List.nil Type) Bool Bool)
+                (Veil.instFieldRepresentationNil Bool)))
+            (Veil.instLawfulFieldRepresentationNilInferInstanceFieldRepresentation Bool)))
+        f (@Eq.symm State.Label f State.Label.locked h))
+    (fun h =>
+      @Eq.ndrec State.Label State.Label.wait_queue_wakers
+        (fun f =>
+          Veil.LawfulFieldRepresentation (State.Label.toDomain process states f)
+            (State.Label.toCodomain process states f) (@FieldConcreteType process states inst_2 inst_3 f)
+            (@instRepForFieldRepresentation process states inst inst_1 inst_2 inst_3 inst_4 inst_5 inst_6 inst_7 f))
+        (@id
+          (Veil.LawfulFieldRepresentation (State.Label.toDomain process states State.Label.wait_queue_wakers)
+            (State.Label.toCodomain process states State.Label.wait_queue_wakers)
+            (@FieldConcreteType process states inst_2 inst_3 State.Label.wait_queue_wakers)
+            (@instRepForFieldRepresentation process states inst inst_1 inst_2 inst_3 inst_4 inst_5 inst_6 inst_7
+              State.Label.wait_queue_wakers))
+          (@inferInstance
+            (Veil.LawfulFieldRepresentation (@List.nil Type) (List process) (List process)
+              (@inferInstance (Veil.FieldRepresentation (@List.nil Type) (List process) (List process))
+                (Veil.instFieldRepresentationNil (List process))))
+            (Veil.instLawfulFieldRepresentationNilInferInstanceFieldRepresentation (List process))))
+        f (@Eq.symm State.Label f State.Label.wait_queue_wakers h))
+    (fun h =>
+      @Eq.ndrec State.Label State.Label.has_woken
+        (fun f =>
+          Veil.LawfulFieldRepresentation (State.Label.toDomain process states f)
+            (State.Label.toCodomain process states f) (@FieldConcreteType process states inst_2 inst_3 f)
+            (@instRepForFieldRepresentation process states inst inst_1 inst_2 inst_3 inst_4 inst_5 inst_6 inst_7 f))
+        (@id
+          (Veil.LawfulFieldRepresentation (State.Label.toDomain process states State.Label.has_woken)
+            (State.Label.toCodomain process states State.Label.has_woken)
+            (@FieldConcreteType process states inst_2 inst_3 State.Label.has_woken)
+            (@instRepForFieldRepresentation process states inst inst_1 inst_2 inst_3 inst_4 inst_5 inst_6 inst_7
+              State.Label.has_woken))
+          (@inferInstance
+            (Veil.LawfulFieldRepresentation (@List.cons Type process (@List.nil Type)) Bool
+              (Std.TreeSet process
+                (@compare process (@instOrdForToDomain' process states inst_2 inst_3 State.Label.has_woken)))
+              (@Veil.instFinsetLikeAsFieldRep process
+                (Std.TreeSet process
+                  (@compare process (@instOrdForToDomain' process states inst_2 inst_3 State.Label.has_woken)))
+                (@List.cons Type process (@List.nil Type))
+                (@Std.TreeSet.instMembership process
+                  (@compare process (@instOrdForToDomain' process states inst_2 inst_3 State.Label.has_woken)))
+                (@Veil.instFinsetLikeTreeSet process
+                  (@compare process (@instOrdForToDomain' process states inst_2 inst_3 State.Label.has_woken)))
+                (@Std.TreeSet.instDecidableMem process
+                  (@compare process (@instOrdForToDomain' process states inst_2 inst_3 State.Label.has_woken)))
+                (@Veil.IteratedProd'.equiv (@List.cons Type process (@List.nil Type)))
+                (@instFinEnumForToDomain process states inst inst_1 State.Label.has_woken)))
+            (@Veil.instFinsetLikeLawfulFieldRep process
+              (Std.TreeSet process
+                (@compare process (@instOrdForToDomain' process states inst_2 inst_3 State.Label.has_woken)))
+              (@List.cons Type process (@List.nil Type)) (fun a b => @FinEnum.decEq process inst a b)
+              (@Std.TreeSet.instMembership process
+                (@compare process (@instOrdForToDomain' process states inst_2 inst_3 State.Label.has_woken)))
+              (@Veil.instFinsetLikeTreeSet process
+                (@compare process (@instOrdForToDomain' process states inst_2 inst_3 State.Label.has_woken)))
+              (@Veil.instLawfulFinsetLikeTreeSetOfLawfulEqCmpOfTransCmp process
+                (@compare process (@instOrdForToDomain' process states inst_2 inst_3 State.Label.has_woken)) inst_4
+                inst_6 fun a b => @FinEnum.decEq process inst a b)
+              (@Std.TreeSet.instDecidableMem process
+                (@compare process (@instOrdForToDomain' process states inst_2 inst_3 State.Label.has_woken)))
+              (@Veil.IteratedProd'.equiv (@List.cons Type process (@List.nil Type)))
+              (@instFinEnumForToDomain process states inst inst_1 State.Label.has_woken))))
+        f (@Eq.symm State.Label f State.Label.has_woken h))
+    (fun h =>
+      @Eq.ndrec State.Label State.Label.pc
+        (fun f =>
+          Veil.LawfulFieldRepresentation (State.Label.toDomain process states f)
+            (State.Label.toCodomain process states f) (@FieldConcreteType process states inst_2 inst_3 f)
+            (@instRepForFieldRepresentation process states inst inst_1 inst_2 inst_3 inst_4 inst_5 inst_6 inst_7 f))
+        (@id
+          (Veil.LawfulFieldRepresentation (State.Label.toDomain process states State.Label.pc)
+            (State.Label.toCodomain process states State.Label.pc)
+            (@FieldConcreteType process states inst_2 inst_3 State.Label.pc)
+            (@instRepForFieldRepresentation process states inst inst_1 inst_2 inst_3 inst_4 inst_5 inst_6 inst_7
+              State.Label.pc))
+          (@inferInstance
+            (Veil.LawfulFieldRepresentation (@List.cons Type process (@List.cons Type states (@List.nil Type))) Bool
+              (Std.TreeSet (Prod process states)
+                (@compare (Prod process states) (@instOrdForToDomain' process states inst_2 inst_3 State.Label.pc)))
+              (@Veil.instFinsetLikeAsFieldRep (Prod process states)
+                (Std.TreeSet (Prod process states)
+                  (@compare (Prod process states) (@instOrdForToDomain' process states inst_2 inst_3 State.Label.pc)))
+                (@List.cons Type process (@List.cons Type states (@List.nil Type)))
+                (@Std.TreeSet.instMembership (Prod process states)
+                  (@compare (Prod process states) (@instOrdForToDomain' process states inst_2 inst_3 State.Label.pc)))
+                (@Veil.instFinsetLikeTreeSet (Prod process states)
+                  (@compare (Prod process states) (@instOrdForToDomain' process states inst_2 inst_3 State.Label.pc)))
+                (@Std.TreeSet.instDecidableMem (Prod process states)
+                  (@compare (Prod process states) (@instOrdForToDomain' process states inst_2 inst_3 State.Label.pc)))
+                (@Veil.IteratedProd'.equiv (@List.cons Type process (@List.cons Type states (@List.nil Type))))
+                (@instFinEnumForToDomain process states inst inst_1 State.Label.pc)))
+            (@Veil.instFinsetLikeLawfulFieldRep (Prod process states)
+              (Std.TreeSet (Prod process states)
+                (@compare (Prod process states) (@instOrdForToDomain' process states inst_2 inst_3 State.Label.pc)))
+              (@List.cons Type process (@List.cons Type states (@List.nil Type)))
+              (fun a b =>
+                @instDecidableEqProd process states (fun a b => @FinEnum.decEq process inst a b)
+                  (fun a b => @FinEnum.decEq states inst_1 a b) a b)
+              (@Std.TreeSet.instMembership (Prod process states)
+                (@compare (Prod process states) (@instOrdForToDomain' process states inst_2 inst_3 State.Label.pc)))
+              (@Veil.instFinsetLikeTreeSet (Prod process states)
+                (@compare (Prod process states) (@instOrdForToDomain' process states inst_2 inst_3 State.Label.pc)))
+              (@Veil.instLawfulFinsetLikeTreeSetOfLawfulEqCmpOfTransCmp (Prod process states)
+                (@compare (Prod process states) (@instOrdForToDomain' process states inst_2 inst_3 State.Label.pc))
+                (@Std.instLawfulEqOrdProd process states inst_2 inst_3 inst_4 inst_5)
+                (@Std.instTransOrdProd process states inst_2 inst_3 inst_6 inst_7) fun a b =>
+                @instDecidableEqProd process states (fun a b => @FinEnum.decEq process inst a b)
+                  (fun a b => @FinEnum.decEq states inst_1 a b) a b)
+              (@Std.TreeSet.instDecidableMem (Prod process states)
+                (@compare (Prod process states) (@instOrdForToDomain' process states inst_2 inst_3 State.Label.pc)))
+              (@Veil.IteratedProd'.equiv (@List.cons Type process (@List.cons Type states (@List.nil Type))))
+              (@instFinEnumForToDomain process states inst inst_1 State.Label.pc))))
+        f (@Eq.symm State.Label f State.Label.pc h))
+    (fun h =>
+      @Eq.ndrec State.Label State.Label.stack
+        (fun f =>
+          Veil.LawfulFieldRepresentation (State.Label.toDomain process states f)
+            (State.Label.toCodomain process states f) (@FieldConcreteType process states inst_2 inst_3 f)
+            (@instRepForFieldRepresentation process states inst inst_1 inst_2 inst_3 inst_4 inst_5 inst_6 inst_7 f))
+        (@id
+          (Veil.LawfulFieldRepresentation (State.Label.toDomain process states State.Label.stack)
+            (State.Label.toCodomain process states State.Label.stack)
+            (@FieldConcreteType process states inst_2 inst_3 State.Label.stack)
+            (@instRepForFieldRepresentation process states inst inst_1 inst_2 inst_3 inst_4 inst_5 inst_6 inst_7
+              State.Label.stack))
+          (@inferInstance
+            (Veil.LawfulFieldRepresentation (@List.cons Type process (@List.nil Type)) (List (Cell states process))
+              (Veil.TotalTreeMap process (List (Cell states process))
+                (@compare process (@instOrdForToDomain' process states inst_2 inst_3 State.Label.stack)))
+              (@Veil.instTotalMapLikeAsFieldRep process
+                (Veil.TotalTreeMap process (List (Cell states process))
+                  (@compare process (@instOrdForToDomain' process states inst_2 inst_3 State.Label.stack)))
+                (@List.cons Type process (@List.nil Type)) (List (Cell states process))
+                (@Veil.instTotalMapLikeTotalTreeMapOfTransCmp (List (Cell states process)) process
+                  (@compare process (@instOrdForToDomain' process states inst_2 inst_3 State.Label.stack)) inst_6)
+                (@Veil.IteratedProd'.equiv (@List.cons Type process (@List.nil Type)))
+                (@instFinEnumForToDomain process states inst inst_1 State.Label.stack)))
+            (@Veil.instTotalMapLikeLawfulFieldRep process
+              (Veil.TotalTreeMap process (List (Cell states process))
+                (@compare process (@instOrdForToDomain' process states inst_2 inst_3 State.Label.stack)))
+              (@List.cons Type process (@List.nil Type)) (List (Cell states process))
+              (fun a b => @FinEnum.decEq process inst a b)
+              (@Veil.instTotalMapLikeTotalTreeMapOfTransCmp (List (Cell states process)) process
+                (@compare process (@instOrdForToDomain' process states inst_2 inst_3 State.Label.stack)) inst_6)
+              (@Veil.instLawfulTotalMapLikeTotalTreeMapOfLawfulEqCmp (List (Cell states process)) process
+                (@compare process (@instOrdForToDomain' process states inst_2 inst_3 State.Label.stack)) inst_4 inst_6
+                fun a b => @FinEnum.decEq process inst a b)
+              (@Veil.IteratedProd'.equiv (@List.cons Type process (@List.nil Type)))
+              (@instFinEnumForToDomain process states inst inst_1 State.Label.stack))))
+        f (@Eq.symm State.Label f State.Label.stack h))
+    (fun h =>
+      @Eq.ndrec State.Label State.Label.waker
+        (fun f =>
+          Veil.LawfulFieldRepresentation (State.Label.toDomain process states f)
+            (State.Label.toCodomain process states f) (@FieldConcreteType process states inst_2 inst_3 f)
+            (@instRepForFieldRepresentation process states inst inst_1 inst_2 inst_3 inst_4 inst_5 inst_6 inst_7 f))
+        (@id
+          (Veil.LawfulFieldRepresentation (State.Label.toDomain process states State.Label.waker)
+            (State.Label.toCodomain process states State.Label.waker)
+            (@FieldConcreteType process states inst_2 inst_3 State.Label.waker)
+            (@instRepForFieldRepresentation process states inst inst_1 inst_2 inst_3 inst_4 inst_5 inst_6 inst_7
+              State.Label.waker))
+          (@inferInstance
+            (Veil.LawfulFieldRepresentation (@List.cons Type process (@List.cons Type process (@List.nil Type))) Bool
+              (Std.TreeSet (Prod process process)
+                (@compare (Prod process process) (@instOrdForToDomain' process states inst_2 inst_3 State.Label.waker)))
+              (@Veil.instFinsetLikeAsFieldRep (Prod process process)
+                (Std.TreeSet (Prod process process)
+                  (@compare (Prod process process)
+                    (@instOrdForToDomain' process states inst_2 inst_3 State.Label.waker)))
+                (@List.cons Type process (@List.cons Type process (@List.nil Type)))
+                (@Std.TreeSet.instMembership (Prod process process)
+                  (@compare (Prod process process)
+                    (@instOrdForToDomain' process states inst_2 inst_3 State.Label.waker)))
+                (@Veil.instFinsetLikeTreeSet (Prod process process)
+                  (@compare (Prod process process)
+                    (@instOrdForToDomain' process states inst_2 inst_3 State.Label.waker)))
+                (@Std.TreeSet.instDecidableMem (Prod process process)
+                  (@compare (Prod process process)
+                    (@instOrdForToDomain' process states inst_2 inst_3 State.Label.waker)))
+                (@Veil.IteratedProd'.equiv (@List.cons Type process (@List.cons Type process (@List.nil Type))))
+                (@instFinEnumForToDomain process states inst inst_1 State.Label.waker)))
+            (@Veil.instFinsetLikeLawfulFieldRep (Prod process process)
+              (Std.TreeSet (Prod process process)
+                (@compare (Prod process process) (@instOrdForToDomain' process states inst_2 inst_3 State.Label.waker)))
+              (@List.cons Type process (@List.cons Type process (@List.nil Type)))
+              (fun a b =>
+                @instDecidableEqProd process process (fun a b => @FinEnum.decEq process inst a b)
+                  (fun a b => @FinEnum.decEq process inst a b) a b)
+              (@Std.TreeSet.instMembership (Prod process process)
+                (@compare (Prod process process) (@instOrdForToDomain' process states inst_2 inst_3 State.Label.waker)))
+              (@Veil.instFinsetLikeTreeSet (Prod process process)
+                (@compare (Prod process process) (@instOrdForToDomain' process states inst_2 inst_3 State.Label.waker)))
+              (@Veil.instLawfulFinsetLikeTreeSetOfLawfulEqCmpOfTransCmp (Prod process process)
+                (@compare (Prod process process) (@instOrdForToDomain' process states inst_2 inst_3 State.Label.waker))
+                (@Std.instLawfulEqOrdProd process process inst_2 inst_2 inst_4 inst_4)
+                (@Std.instTransOrdProd process process inst_2 inst_2 inst_6 inst_6) fun a b =>
+                @instDecidableEqProd process process (fun a b => @FinEnum.decEq process inst a b)
+                  (fun a b => @FinEnum.decEq process inst a b) a b)
+              (@Std.TreeSet.instDecidableMem (Prod process process)
+                (@compare (Prod process process) (@instOrdForToDomain' process states inst_2 inst_3 State.Label.waker)))
+              (@Veil.IteratedProd'.equiv (@List.cons Type process (@List.cons Type process (@List.nil Type))))
+              (@instFinEnumForToDomain process states inst inst_1 State.Label.waker))))
+        f (@Eq.symm State.Label f State.Label.waker h))
+    (@Eq.refl State.Label f)
+
+gen_NextAct
+-- attribute [local dsimpFieldRepresentationGet, local dsimpFieldRepresentationSet] instFinEnumForToDomain in
+-- #specialize_nextact with FieldConcreteType
+--   injection_begin[FinEnum
+--       process][FinEnum
+--       states][Hashable
+--       process][Hashable
+--       states][Ord
+--       process][Ord
+--       states][Std.LawfulEqCmp
+--       (Ord.compare (self :=
+--         inferInstanceAs
+--           (Ord
+--             process)))][Std.LawfulEqCmp
+--       (Ord.compare (self :=
+--         inferInstanceAs
+--           (Ord
+--             states)))][Std.TransCmp
+--       (Ord.compare (self :=
+--         inferInstanceAs
+--           (Ord
+--             process)))][Std.TransCmp
+--       (Ord.compare (self :=
+--         inferInstanceAs
+--           (Ord
+--             states)))][Std.LawfulEqCmp
+--       (Ord.compare (self :=
+--         inferInstanceAs
+--           (Ord
+--             (Bool))))][Std.TransCmp
+--       (Ord.compare (self :=
+--         inferInstanceAs
+--           (Ord
+--             (Bool))))][Std.LawfulEqCmp
+--       (Ord.compare (self :=
+--         inferInstanceAs
+--           (Ord
+--             (List
+--               process))))][Std.TransCmp
+--       (Ord.compare (self :=
+--         inferInstanceAs
+--           (Ord
+--             (List
+--               process))))][Std.LawfulEqCmp
+--       (Ord.compare (self :=
+--         inferInstanceAs
+--           (Ord
+--             (process))))][Std.TransCmp
+--       (Ord.compare (self :=
+--         inferInstanceAs
+--           (Ord
+--             (process))))][Std.LawfulEqCmp
+--       (Ord.compare (self :=
+--         inferInstanceAs
+--           (Ord
+--             (process ×
+--               (states)))))][Std.TransCmp
+--       (Ord.compare (self :=
+--         inferInstanceAs
+--           (Ord
+--             (process ×
+--               (states)))))][Std.LawfulEqCmp
+--       (Ord.compare (self :=
+--         inferInstanceAs
+--           (Ord
+--             (process ×
+--               (process)))))][Std.TransCmp
+--       (Ord.compare (self := inferInstanceAs (Ord (process × (process)))))]
+--       injection_end=>NextAct'
+
+
+gen_executable_NextAct
+
+
+-- deriving_enum_instance_for states
+-- deriving_ord_hashable_for_enum states
+-- deriving_propCmp_for_enum states
+deriving_Enum_Insts
+
+
+-- instance {process states : Type}
+-- [states_ord: Ord states] [process_ord: Ord process]
+-- : Std.OrientedCmp (Ord.compare (self := inferInstanceAs (Ord (Cell states process)))) := by
+--   apply Std.OrientedCmp.mk
+--   unfold compare inferInstanceAs
+--   intro a b; cases a <;>
+--     cases b <;> rfl
+
+-- instance [FinEnum states] : Std.OrientedCmp (Ord.compare (self := inferInstanceAs (Ord states))) := by
+--   apply Std.OrientedCmp.mk
+--   unfold compare inferInstanceAs instOrdstates
+--   intro a b; cases a <;>
+--     cases b <;> rfl
+
+-- instance : Std.TransCmp (Ord.compare (self := inferInstanceAs (Ord states))) := by
+--   apply Std.TransCmp.mk
+--   unfold compare inferInstanceAs instOrdstates
+--   decide
+
+-- instance : Std.LawfulEqCmp (Ord.compare (self := inferInstanceAs (Ord states))) := by
+--   apply Std.LawfulEqCmp.mk
+--   unfold compare inferInstanceAs
+--   intro a b; cases a <;>
+--     cases b <;> simp <;> decide
+
+
+
+-- instance (α β : Type)
+-- [a_ord: Ord α]
+-- [b_ord: Ord β]
+-- [cell_ord : Ord (Cell α β)]
+-- [a_oriented: Std.OrientedCmp (Ord.compare (self := a_ord))]
+-- [b_oriented: Std.OrientedCmp (Ord.compare (self := b_ord))]
+--  : Std.OrientedCmp (Ord.compare (self := inferInstanceAs (Ord (Cell α β)))) := by
+--   apply Std.OrientedCmp.mk
+--   unfold compare inferInstanceAs
+--   intro a b
+--   cases a <;>
+--     cases b <;>
+--     unfold ordCell
+
+#Concretize (Fin 3), states
+
+deriving_BEqHashable_ConcreteState
+simple_deriving_repr_for' State
+deriving instance Repr for Label
+deriving instance Inhabited for Theory
+deriving_toJson_for_state
+deriving_DecidableProps_state
+
+
+
+def view (st : StateConcrete) := hash st
+
+
+def modelCheckerResult' :=
+  (runModelCheckerx initVeilMultiExecM nextVeilMultiExecM labelList (fun ρ σ => mutual_exclusion ρ σ) ((fun ρ σ => allDone ρ σ)) {none := 0} view).snd
+
+
+open Lean
+
+def statesJson : Json :=
+  toJson (recoverTrace initVeilMultiExecM nextVeilMultiExecM {none := 0} (collectTrace' modelCheckerResult'))
+
+#check statesJson
+
+#eval statesJson
+open ProofWidgets
+open scoped ProofWidgets.Jsx
+#html <ModelCheckerView trace={statesJson} layout={"vertical"} />
+
+end Mutex
