Veil/Core/Tools/Checker/Concrete/Runlib.lean
@@ -1,0 +1,165 @@
+import Std
+import Veil.Frontend.Std
+import Veil.Core.Tools.Checker.Concrete.State
+import Veil.Frontend.DSL.Infra.GenericInterface
+
+
+/--
+`BEq` instances for `Std.TreeMap` and `Std.TreeSet`.
+
+We need `BEq` instance, as we sometimes hope to store them in `HashSet` or `HashMap`,
+e.g., debugging, when we hope to store the complete information of a state `σᵣ`.
+-/
+instance [Ord α] [BEq α]: BEq (Std.TreeSet α) where
+  beq s1 s2 :=
+    s1.toArray == s2.toArray
+
+instance [Ord α] [BEq α] [BEq β]: BEq (Std.TreeMap α β) where
+  beq s1 s2 :=
+    s1.toArray == s2.toArray
+
+instance [Ord α] [BEq α] [BEq β]: BEq (Veil.TotalTreeMap α β) where
+  beq s1 s2 :=
+    s1.val.toArray == s2.val.toArray
+
+
+/--
+`Hashable` instances for `Std.TreeMap` and `Std.TreeSet`
+
+We always need `Hashable` instance. When we run the model checker,
+we always store the hashable value of state representation `σᵣ` in `HashSet`.
+-/
+instance [Hashable α] [BEq α] [Ord α]: Hashable (Std.TreeSet α) where
+  hash s := hash s.toArray
+
+instance [Hashable α] [BEq α] [Ord α]: Hashable (Std.TreeSet α) where
+  hash := fun s => hash s.toArray
+
+instance [Ord α] [Hashable α] [Hashable β] : Hashable (Std.TreeMap α β) where
+  hash s := hash s.toArray
+
+instance [Ord α] [Hashable α] [Hashable β]: Hashable (Veil.TotalTreeMap α β) where
+  hash s := hash s.val.toArray
+
+
+/--
+`Ord` instances for `Std.TreeMap` and `Std.TreeSet`
+
+If we want to use `symmetric reduction` in model checking, we need `Ord` instances
+to make the states comparable.
+ -/
+instance [Ord α] [Ord β] : Ord (α × β) where
+  compare x y := match x, y with
+    | (a, b), (a', b') => compare a a' |>.then (compare b b')
+
+instance [Ord α] : Ord (Std.TreeSet α) where
+  compare s1 s2 := compare s1.toArray s2.toArray
+
+instance [Ord α] [Ord β] : Ord (Std.TreeMap α β) where
+  compare s1 s2 := compare s1.toArray s2.toArray
+
+instance [Ord α] [Ord β]: Ord (Veil.TotalTreeMap α β) where
+  compare s1 s2 := compare s1.val.toArray s2.val.toArray
+
+
+/- `ToJson` instances -/
+open Lean
+instance [Repr α]: ToJson α where
+  toJson := fun a => Json.str (toString (repr a))
+
+instance jsonOfTuple [ToJson α] [ToJson β]: ToJson (α × β) where
+  toJson := fun ⟨a, b⟩ => Json.arr #[toJson a, toJson b]
+
+instance jsonOfList [ToJson α]: ToJson (List α) where
+  toJson := fun xs => Json.arr (xs.toArray.map toJson)
+
+instance jsonOfTreeSet [Ord α] [ToJson α] : ToJson (Std.TreeSet α) where
+  toJson s := Json.arr <| s.toArray.map toJson
+
+instance jsonOfTreeMap [Ord α] [ToJson α] [ToJson β] : ToJson (Std.TreeMap α β) where
+  toJson m := Json.arr <| m.toArray.map (fun (k, v) => Json.arr #[toJson k, toJson v])
+
+instance jsonOfTotalTreeMap [Ord α] [ToJson α] [ToJson β] : ToJson (Veil.TotalTreeMap α β) where
+  toJson m := Json.arr <| m.val.toArray.map (fun (k, v) => Json.arr #[toJson k, toJson v])
+
+instance jsonOfTrace {σₛ κ : Type} [ToJson σₛ] [ToJson κ] : ToJson (Trace σₛ κ) where
+  toJson := fun tr =>
+    let states : Array Json :=
+      #[ Json.mkObj [("index", toJson 0),
+        ("fields", toJson tr.start),
+        ("action", "after_init") ]] ++
+      (tr.steps.toArray.mapIdx (fun i st =>
+        let idx := i + 1
+        Json.mkObj [("index", toJson idx),
+        ("fields", toJson st.next),
+        ("action", toJson st.label)]
+      ))
+    Json.arr states
+
+
+
+
+instance (n : Nat): TotalOrderWithZero (Fin n.succ) where
+  le := fun x y => x.val ≤ y.val
+  le_refl := by simp
+  le_trans := by simp ; omega
+  le_antisymm := by simp ; omega
+  le_total := by simp ; omega
+  zero := ⟨0, by simp⟩
+  zero_le := by simp
+
+
+instance (n : Nat) : DecidableRel (TotalOrderWithZero.le (t := Fin n.succ)) := by
+  dsimp [TotalOrderWithZero.le]
+  infer_instance_for_iterated_prod
+
+
+-- instance [Ord α]
+--   : Ord (FieldConcreteType α states State.Label.locked) := by
+--   dsimp only [FieldConcreteType, State.Label.toCodomain, State.Label.toDomain, Veil.IteratedProd'];
+--   infer_instance_for_iterated_prod
+
+-- instance [Ord α]
+--   : Ord (FieldConcreteType α states State.Label.wait_queue_wakers) := by
+--   dsimp only [FieldConcreteType, State.Label.toCodomain, State.Label.toDomain, Veil.IteratedProd'];
+--   infer_instance_for_iterated_prod
+
+-- instance [Ord α]
+--   : Ord (FieldConcreteType α states State.Label.locked) := by
+--   dsimp only [FieldConcreteType, State.Label.toCodomain, State.Label.toDomain, Veil.IteratedProd'];
+--   infer_instance_for_iterated_prod
+
+-- instance [Ord α]
+--   : Ord (FieldConcreteType α states State.Label.has_woken) := by
+--   dsimp only [FieldConcreteType, State.Label.toCodomain, State.Label.toDomain, Veil.IteratedProd'];
+--   infer_instance_for_iterated_prod
+
+-- instance [Ord α]
+--   : Ord (FieldConcreteType α states State.Label.pc) := by
+--   dsimp only [FieldConcreteType, State.Label.toCodomain, State.Label.toDomain, Veil.IteratedProd'];
+--   infer_instance_for_iterated_prod
+
+-- instance [Ord α]
+--   : Ord (FieldConcreteType α states State.Label.stack_pc) := by
+--   dsimp only [FieldConcreteType, State.Label.toCodomain, State.Label.toDomain, Veil.IteratedProd'];
+--   infer_instance_for_iterated_prod
+
+-- instance [Ord α]
+--   : Ord (FieldConcreteType α states State.Label.stack_waker) := by
+--   dsimp only [FieldConcreteType, State.Label.toCodomain, State.Label.toDomain, Veil.IteratedProd'];
+--   infer_instance_for_iterated_prod
+
+-- instance [Ord α]
+--   : Ord (FieldConcreteType α states State.Label.waker) := by
+--   dsimp only [FieldConcreteType, State.Label.toCodomain, State.Label.toDomain, Veil.IteratedProd'];
+--   infer_instance_for_iterated_prod
+
+-- instance: Ord StateConcrete where
+--   compare a b :=
+--     compare a.locked b.locked |>.then
+--     (compare a.wait_queue_wakers b.wait_queue_wakers) |>.then
+--     (compare a.has_woken b.has_woken) |>.then
+--     (compare a.pc b.pc) |>.then
+--     (compare a.stack_pc b.stack_pc) |>.then
+--     (compare a.stack_waker b.stack_waker) |>.then
+--     (compare a.waker b.waker)
